restored error prop

libcrux-ml-dsa/proofs/fstar/extraction/Libcrux_ml_dsa.Simd.Avx2.Encoding.Error.fst
@@ -12,7 +12,7 @@ let deserialize_to_unsigned_when_eta_is_2_ (bytes: t_Slice u8) =
       in
       ()
   in
-  let bytes_in_simd_unit:Libcrux_intrinsics.Avx2_extract.t_Vec256 =
+  let bytes_in_simd_unit:u8 =
     Libcrux_intrinsics.Avx2_extract.mm256_set_epi32 (cast (bytes.[ sz 2 ] <: u8) <: i32)
       (cast (bytes.[ sz 2 ] <: u8) <: i32)
       (((cast (bytes.[ sz 2 ] <: u8) <: i32) <<! 8l <: i32) |. (cast (bytes.[ sz 1 ] <: u8) <: i32)
@@ -26,17 +26,15 @@ let deserialize_to_unsigned_when_eta_is_2_ (bytes: t_Slice u8) =
       (cast (bytes.[ sz 0 ] <: u8) <: i32)
       (cast (bytes.[ sz 0 ] <: u8) <: i32)
   in
-  let coefficients:Libcrux_intrinsics.Avx2_extract.t_Vec256 =
+  let coefficients:u8 =
     Libcrux_intrinsics.Avx2_extract.mm256_srlv_epi32 bytes_in_simd_unit
-      (Libcrux_intrinsics.Avx2_extract.mm256_set_epi32 5l 2l 7l 4l 1l 6l 3l 0l
-        <:
-        Libcrux_intrinsics.Avx2_extract.t_Vec256)
+      (Libcrux_intrinsics.Avx2_extract.mm256_set_epi32 5l 2l 7l 4l 1l 6l 3l 0l <: u8)
   in
   Libcrux_intrinsics.Avx2_extract.mm256_and_si256 coefficients
     (Libcrux_intrinsics.Avx2_extract.mm256_set1_epi32 deserialize_to_unsigned_when_eta_is_2___COEFFICIENT_MASK
 
       <:
-      Libcrux_intrinsics.Avx2_extract.t_Vec256)
+      u8)
 
 let deserialize_to_unsigned_when_eta_is_4_ (bytes: t_Slice u8) =
   let _:Prims.unit =
@@ -47,7 +45,7 @@ let deserialize_to_unsigned_when_eta_is_4_ (bytes: t_Slice u8) =
       in
       ()
   in
-  let bytes_in_simd_unit:Libcrux_intrinsics.Avx2_extract.t_Vec256 =
+  let bytes_in_simd_unit:u8 =
     Libcrux_intrinsics.Avx2_extract.mm256_set_epi32 (cast (bytes.[ sz 3 ] <: u8) <: i32)
       (cast (bytes.[ sz 3 ] <: u8) <: i32)
       (cast (bytes.[ sz 2 ] <: u8) <: i32)
@@ -57,17 +55,15 @@ let deserialize_to_unsigned_when_eta_is_4_ (bytes: t_Slice u8) =
       (cast (bytes.[ sz 0 ] <: u8) <: i32)
       (cast (bytes.[ sz 0 ] <: u8) <: i32)
   in
-  let coefficients:Libcrux_intrinsics.Avx2_extract.t_Vec256 =
+  let coefficients:u8 =
     Libcrux_intrinsics.Avx2_extract.mm256_srlv_epi32 bytes_in_simd_unit
-      (Libcrux_intrinsics.Avx2_extract.mm256_set_epi32 4l 0l 4l 0l 4l 0l 4l 0l
-        <:
-        Libcrux_intrinsics.Avx2_extract.t_Vec256)
+      (Libcrux_intrinsics.Avx2_extract.mm256_set_epi32 4l 0l 4l 0l 4l 0l 4l 0l <: u8)
   in
   Libcrux_intrinsics.Avx2_extract.mm256_and_si256 coefficients
     (Libcrux_intrinsics.Avx2_extract.mm256_set1_epi32 deserialize_to_unsigned_when_eta_is_4___COEFFICIENT_MASK
 
       <:
-      Libcrux_intrinsics.Avx2_extract.t_Vec256)
+      u8)
 
 let deserialize_to_unsigned (v_ETA: usize) (serialized: t_Slice u8) =
   match cast (v_ETA <: usize) <: u8 with
@@ -80,67 +76,56 @@ let deserialize_to_unsigned (v_ETA: usize) (serialized: t_Slice u8) =
         Rust_primitives.Hax.t_Never)
 
 let deserialize (v_ETA: usize) (serialized: t_Slice u8) =
-  let unsigned:Libcrux_intrinsics.Avx2_extract.t_Vec256 =
-    deserialize_to_unsigned v_ETA serialized
-  in
+  let unsigned:u8 = deserialize_to_unsigned v_ETA serialized in
   Libcrux_intrinsics.Avx2_extract.mm256_sub_epi32 (Libcrux_intrinsics.Avx2_extract.mm256_set1_epi32 (
           cast (v_ETA <: usize) <: i32)
       <:
-      Libcrux_intrinsics.Avx2_extract.t_Vec256)
+      u8)
     unsigned
 
-let serialize_when_eta_is_2_
-      (v_OUTPUT_SIZE: usize)
-      (simd_unit: Libcrux_intrinsics.Avx2_extract.t_Vec256)
-     =
+let serialize_when_eta_is_2_ (v_OUTPUT_SIZE: usize) (simd_unit: u8) =
   let serialized:t_Array u8 (sz 16) = Rust_primitives.Hax.repeat 0uy (sz 16) in
-  let simd_unit_shifted:Libcrux_intrinsics.Avx2_extract.t_Vec256 =
+  let simd_unit_shifted:u8 =
     Libcrux_intrinsics.Avx2_extract.mm256_sub_epi32 (Libcrux_intrinsics.Avx2_extract.mm256_set1_epi32
           serialize_when_eta_is_2___ETA
         <:
-        Libcrux_intrinsics.Avx2_extract.t_Vec256)
+        u8)
       simd_unit
   in
-  let adjacent_2_combined:Libcrux_intrinsics.Avx2_extract.t_Vec256 =
+  let adjacent_2_combined:u8 =
     Libcrux_intrinsics.Avx2_extract.mm256_sllv_epi32 simd_unit_shifted
-      (Libcrux_intrinsics.Avx2_extract.mm256_set_epi32 0l 29l 0l 29l 0l 29l 0l 29l
-        <:
-        Libcrux_intrinsics.Avx2_extract.t_Vec256)
+      (Libcrux_intrinsics.Avx2_extract.mm256_set_epi32 0l 29l 0l 29l 0l 29l 0l 29l <: u8)
   in
-  let adjacent_2_combined:Libcrux_intrinsics.Avx2_extract.t_Vec256 =
+  let adjacent_2_combined:u8 =
     Libcrux_intrinsics.Avx2_extract.mm256_srli_epi64 29l adjacent_2_combined
   in
-  let adjacent_4_combined:Libcrux_intrinsics.Avx2_extract.t_Vec256 =
+  let adjacent_4_combined:u8 =
     Libcrux_intrinsics.Avx2_extract.mm256_shuffle_epi8 adjacent_2_combined
       (Libcrux_intrinsics.Avx2_extract.mm256_set_epi8 (-1y) (-1y) (-1y) (-1y) (-1y) (-1y) (-1y)
           (-1y) (-1y) (-1y) (-1y) (-1y) (-1y) 8y (-1y) 0y (-1y) (-1y) (-1y) (-1y) (-1y) (-1y) (-1y)
           (-1y) (-1y) (-1y) (-1y) (-1y) (-1y) 8y (-1y) 0y
         <:
-        Libcrux_intrinsics.Avx2_extract.t_Vec256)
+        u8)
   in
-  let adjacent_4_combined:Libcrux_intrinsics.Avx2_extract.t_Vec256 =
+  let adjacent_4_combined:u8 =
     Libcrux_intrinsics.Avx2_extract.mm256_madd_epi16 adjacent_4_combined
       (Libcrux_intrinsics.Avx2_extract.mm256_set_epi16 0s 0s 0s 0s 0s 0s (1s <<! 6l <: i16) 1s 0s 0s
           0s 0s 0s 0s (1s <<! 6l <: i16) 1s
         <:
-        Libcrux_intrinsics.Avx2_extract.t_Vec256)
+        u8)
   in
-  let adjacent_6_combined:Libcrux_intrinsics.Avx2_extract.t_Vec256 =
+  let adjacent_6_combined:u8 =
     Libcrux_intrinsics.Avx2_extract.mm256_permutevar8x32_epi32 adjacent_4_combined
-      (Libcrux_intrinsics.Avx2_extract.mm256_set_epi32 0l 0l 0l 0l 0l 0l 4l 0l
-        <:
-        Libcrux_intrinsics.Avx2_extract.t_Vec256)
+      (Libcrux_intrinsics.Avx2_extract.mm256_set_epi32 0l 0l 0l 0l 0l 0l 4l 0l <: u8)
   in
-  let adjacent_6_combined:Libcrux_intrinsics.Avx2_extract.t_Vec128 =
+  let adjacent_6_combined:u8 =
     Libcrux_intrinsics.Avx2_extract.mm256_castsi256_si128 adjacent_6_combined
   in
-  let adjacent_6_combined:Libcrux_intrinsics.Avx2_extract.t_Vec128 =
+  let adjacent_6_combined:u8 =
     Libcrux_intrinsics.Avx2_extract.mm_sllv_epi32 adjacent_6_combined
-      (Libcrux_intrinsics.Avx2_extract.mm_set_epi32 0l 0l 0l 20l
-        <:
-        Libcrux_intrinsics.Avx2_extract.t_Vec128)
+      (Libcrux_intrinsics.Avx2_extract.mm_set_epi32 0l 0l 0l 20l <: u8)
   in
-  let adjacent_6_combined:Libcrux_intrinsics.Avx2_extract.t_Vec128 =
+  let adjacent_6_combined:u8 =
     Libcrux_intrinsics.Avx2_extract.mm_srli_epi64 20l adjacent_6_combined
   in
   let serialized:t_Array u8 (sz 16) =
@@ -173,42 +158,35 @@ let serialize_when_eta_is_2_
       <:
       Core.Result.t_Result (t_Array u8 v_OUTPUT_SIZE) Core.Array.t_TryFromSliceError)
 
-let serialize_when_eta_is_4_
-      (v_OUTPUT_SIZE: usize)
-      (simd_unit: Libcrux_intrinsics.Avx2_extract.t_Vec256)
-     =
+let serialize_when_eta_is_4_ (v_OUTPUT_SIZE: usize) (simd_unit: u8) =
   let serialized:t_Array u8 (sz 16) = Rust_primitives.Hax.repeat 0uy (sz 16) in
-  let simd_unit_shifted:Libcrux_intrinsics.Avx2_extract.t_Vec256 =
+  let simd_unit_shifted:u8 =
     Libcrux_intrinsics.Avx2_extract.mm256_sub_epi32 (Libcrux_intrinsics.Avx2_extract.mm256_set1_epi32
           serialize_when_eta_is_4___ETA
         <:
-        Libcrux_intrinsics.Avx2_extract.t_Vec256)
+        u8)
       simd_unit
   in
-  let adjacent_2_combined:Libcrux_intrinsics.Avx2_extract.t_Vec256 =
+  let adjacent_2_combined:u8 =
     Libcrux_intrinsics.Avx2_extract.mm256_sllv_epi32 simd_unit_shifted
-      (Libcrux_intrinsics.Avx2_extract.mm256_set_epi32 0l 28l 0l 28l 0l 28l 0l 28l
-        <:
-        Libcrux_intrinsics.Avx2_extract.t_Vec256)
+      (Libcrux_intrinsics.Avx2_extract.mm256_set_epi32 0l 28l 0l 28l 0l 28l 0l 28l <: u8)
   in
-  let adjacent_2_combined:Libcrux_intrinsics.Avx2_extract.t_Vec256 =
+  let adjacent_2_combined:u8 =
     Libcrux_intrinsics.Avx2_extract.mm256_srli_epi64 28l adjacent_2_combined
   in
-  let adjacent_4_combined:Libcrux_intrinsics.Avx2_extract.t_Vec256 =
+  let adjacent_4_combined:u8 =
     Libcrux_intrinsics.Avx2_extract.mm256_permutevar8x32_epi32 adjacent_2_combined
-      (Libcrux_intrinsics.Avx2_extract.mm256_set_epi32 0l 0l 0l 0l 6l 2l 4l 0l
-        <:
-        Libcrux_intrinsics.Avx2_extract.t_Vec256)
+      (Libcrux_intrinsics.Avx2_extract.mm256_set_epi32 0l 0l 0l 0l 6l 2l 4l 0l <: u8)
   in
-  let adjacent_4_combined:Libcrux_intrinsics.Avx2_extract.t_Vec128 =
+  let adjacent_4_combined:u8 =
     Libcrux_intrinsics.Avx2_extract.mm256_castsi256_si128 adjacent_4_combined
   in
-  let adjacent_4_combined:Libcrux_intrinsics.Avx2_extract.t_Vec128 =
+  let adjacent_4_combined:u8 =
     Libcrux_intrinsics.Avx2_extract.mm_shuffle_epi8 adjacent_4_combined
       (Libcrux_intrinsics.Avx2_extract.mm_set_epi8 240uy 240uy 240uy 240uy 240uy 240uy 240uy 240uy
           240uy 240uy 240uy 240uy 12uy 4uy 8uy 0uy
         <:
-        Libcrux_intrinsics.Avx2_extract.t_Vec128)
+        u8)
   in
   let serialized:t_Array u8 (sz 16) =
     Rust_primitives.Hax.Monomorphized_update_at.update_at_range serialized
@@ -240,7 +218,7 @@ let serialize_when_eta_is_4_
       <:
       Core.Result.t_Result (t_Array u8 v_OUTPUT_SIZE) Core.Array.t_TryFromSliceError)
 
-let serialize (v_OUTPUT_SIZE: usize) (simd_unit: Libcrux_intrinsics.Avx2_extract.t_Vec256) =
+let serialize (v_OUTPUT_SIZE: usize) (simd_unit: u8) =
   match cast (v_OUTPUT_SIZE <: usize) <: u8 with
   | 3uy -> serialize_when_eta_is_2_ v_OUTPUT_SIZE simd_unit
   | 4uy -> serialize_when_eta_is_4_ v_OUTPUT_SIZE simd_unit
