libcrux-ml-dsa/proofs/fstar/extraction/Libcrux_ml_dsa.Simd.Avx2.Encoding.Gamma1.fst
@@ -12,7 +12,7 @@ let deserialize_when_gamma1_is_2_pow_17_ (serialized: t_Slice u8) =
       in
       ()
   in
-  let serialized_lower:Libcrux_intrinsics.Avx2_extract.t_Vec128 =
+  let serialized_lower:u8 =
     Libcrux_intrinsics.Avx2_extract.mm_loadu_si128 (serialized.[ {
             Core.Ops.Range.f_start = sz 0;
             Core.Ops.Range.f_end = sz 16
@@ -22,7 +22,7 @@ let deserialize_when_gamma1_is_2_pow_17_ (serialized: t_Slice u8) =
         <:
         t_Slice u8)
   in
-  let serialized_upper:Libcrux_intrinsics.Avx2_extract.t_Vec128 =
+  let serialized_upper:u8 =
     Libcrux_intrinsics.Avx2_extract.mm_loadu_si128 (serialized.[ {
             Core.Ops.Range.f_start = sz 2;
             Core.Ops.Range.f_end = sz 18
@@ -32,33 +32,31 @@ let deserialize_when_gamma1_is_2_pow_17_ (serialized: t_Slice u8) =
         <:
         t_Slice u8)
   in
-  let serialized:Libcrux_intrinsics.Avx2_extract.t_Vec256 =
+  let serialized:u8 =
     Libcrux_intrinsics.Avx2_extract.mm256_set_m128i serialized_upper serialized_lower
   in
-  let coefficients:Libcrux_intrinsics.Avx2_extract.t_Vec256 =
+  let coefficients:u8 =
     Libcrux_intrinsics.Avx2_extract.mm256_shuffle_epi8 serialized
       (Libcrux_intrinsics.Avx2_extract.mm256_set_epi8 (-1y) 15y 14y 13y (-1y) 13y 12y 11y (-1y) 11y
           10y 9y (-1y) 9y 8y 7y (-1y) 8y 7y 6y (-1y) 6y 5y 4y (-1y) 4y 3y 2y (-1y) 2y 1y 0y
         <:
-        Libcrux_intrinsics.Avx2_extract.t_Vec256)
+        u8)
   in
-  let coefficients:Libcrux_intrinsics.Avx2_extract.t_Vec256 =
+  let coefficients:u8 =
     Libcrux_intrinsics.Avx2_extract.mm256_srlv_epi32 coefficients
-      (Libcrux_intrinsics.Avx2_extract.mm256_set_epi32 6l 4l 2l 0l 6l 4l 2l 0l
-        <:
-        Libcrux_intrinsics.Avx2_extract.t_Vec256)
+      (Libcrux_intrinsics.Avx2_extract.mm256_set_epi32 6l 4l 2l 0l 6l 4l 2l 0l <: u8)
   in
-  let coefficients:Libcrux_intrinsics.Avx2_extract.t_Vec256 =
+  let coefficients:u8 =
     Libcrux_intrinsics.Avx2_extract.mm256_and_si256 coefficients
       (Libcrux_intrinsics.Avx2_extract.mm256_set1_epi32 deserialize_when_gamma1_is_2_pow_17___GAMMA1_TIMES_2_MASK
 
         <:
-        Libcrux_intrinsics.Avx2_extract.t_Vec256)
+        u8)
   in
   Libcrux_intrinsics.Avx2_extract.mm256_sub_epi32 (Libcrux_intrinsics.Avx2_extract.mm256_set1_epi32 deserialize_when_gamma1_is_2_pow_17___GAMMA1
 
       <:
-      Libcrux_intrinsics.Avx2_extract.t_Vec256)
+      u8)
     coefficients
 
 let deserialize_when_gamma1_is_2_pow_19_ (serialized: t_Slice u8) =
@@ -70,7 +68,7 @@ let deserialize_when_gamma1_is_2_pow_19_ (serialized: t_Slice u8) =
       in
       ()
   in
-  let serialized_lower:Libcrux_intrinsics.Avx2_extract.t_Vec128 =
+  let serialized_lower:u8 =
     Libcrux_intrinsics.Avx2_extract.mm_loadu_si128 (serialized.[ {
             Core.Ops.Range.f_start = sz 0;
             Core.Ops.Range.f_end = sz 16
@@ -80,7 +78,7 @@ let deserialize_when_gamma1_is_2_pow_19_ (serialized: t_Slice u8) =
         <:
         t_Slice u8)
   in
-  let serialized_upper:Libcrux_intrinsics.Avx2_extract.t_Vec128 =
+  let serialized_upper:u8 =
     Libcrux_intrinsics.Avx2_extract.mm_loadu_si128 (serialized.[ {
             Core.Ops.Range.f_start = sz 4;
             Core.Ops.Range.f_end = sz 20
@@ -90,33 +88,31 @@ let deserialize_when_gamma1_is_2_pow_19_ (serialized: t_Slice u8) =
         <:
         t_Slice u8)
   in
-  let serialized:Libcrux_intrinsics.Avx2_extract.t_Vec256 =
+  let serialized:u8 =
     Libcrux_intrinsics.Avx2_extract.mm256_set_m128i serialized_upper serialized_lower
   in
-  let coefficients:Libcrux_intrinsics.Avx2_extract.t_Vec256 =
+  let coefficients:u8 =
     Libcrux_intrinsics.Avx2_extract.mm256_shuffle_epi8 serialized
       (Libcrux_intrinsics.Avx2_extract.mm256_set_epi8 (-1y) 15y 14y 13y (-1y) 13y 12y 11y (-1y) 10y
           9y 8y (-1y) 8y 7y 6y (-1y) 9y 8y 7y (-1y) 7y 6y 5y (-1y) 4y 3y 2y (-1y) 2y 1y 0y
         <:
-        Libcrux_intrinsics.Avx2_extract.t_Vec256)
+        u8)
   in
-  let coefficients:Libcrux_intrinsics.Avx2_extract.t_Vec256 =
+  let coefficients:u8 =
     Libcrux_intrinsics.Avx2_extract.mm256_srlv_epi32 coefficients
-      (Libcrux_intrinsics.Avx2_extract.mm256_set_epi32 4l 0l 4l 0l 4l 0l 4l 0l
-        <:
-        Libcrux_intrinsics.Avx2_extract.t_Vec256)
+      (Libcrux_intrinsics.Avx2_extract.mm256_set_epi32 4l 0l 4l 0l 4l 0l 4l 0l <: u8)
   in
-  let coefficients:Libcrux_intrinsics.Avx2_extract.t_Vec256 =
+  let coefficients:u8 =
     Libcrux_intrinsics.Avx2_extract.mm256_and_si256 coefficients
       (Libcrux_intrinsics.Avx2_extract.mm256_set1_epi32 deserialize_when_gamma1_is_2_pow_19___GAMMA1_TIMES_2_MASK
 
         <:
-        Libcrux_intrinsics.Avx2_extract.t_Vec256)
+        u8)
   in
   Libcrux_intrinsics.Avx2_extract.mm256_sub_epi32 (Libcrux_intrinsics.Avx2_extract.mm256_set1_epi32 deserialize_when_gamma1_is_2_pow_19___GAMMA1
 
       <:
-      Libcrux_intrinsics.Avx2_extract.t_Vec256)
+      u8)
     coefficients
 
 let deserialize (v_GAMMA1_EXPONENT: usize) (serialized: t_Slice u8) =
@@ -129,45 +125,36 @@ let deserialize (v_GAMMA1_EXPONENT: usize) (serialized: t_Slice u8) =
         <:
         Rust_primitives.Hax.t_Never)
 
-let serialize_when_gamma1_is_2_pow_17_
-      (v_OUTPUT_SIZE: usize)
-      (simd_unit: Libcrux_intrinsics.Avx2_extract.t_Vec256)
-     =
+let serialize_when_gamma1_is_2_pow_17_ (v_OUTPUT_SIZE: usize) (simd_unit: u8) =
   let serialized:t_Array u8 (sz 32) = Rust_primitives.Hax.repeat 0uy (sz 32) in
-  let simd_unit_shifted:Libcrux_intrinsics.Avx2_extract.t_Vec256 =
+  let simd_unit_shifted:u8 =
     Libcrux_intrinsics.Avx2_extract.mm256_sub_epi32 (Libcrux_intrinsics.Avx2_extract.mm256_set1_epi32
           serialize_when_gamma1_is_2_pow_17___GAMMA1
         <:
-        Libcrux_intrinsics.Avx2_extract.t_Vec256)
+        u8)
       simd_unit
   in
-  let adjacent_2_combined:Libcrux_intrinsics.Avx2_extract.t_Vec256 =
+  let adjacent_2_combined:u8 =
     Libcrux_intrinsics.Avx2_extract.mm256_sllv_epi32 simd_unit_shifted
-      (Libcrux_intrinsics.Avx2_extract.mm256_set_epi32 0l 14l 0l 14l 0l 14l 0l 14l
-        <:
-        Libcrux_intrinsics.Avx2_extract.t_Vec256)
+      (Libcrux_intrinsics.Avx2_extract.mm256_set_epi32 0l 14l 0l 14l 0l 14l 0l 14l <: u8)
   in
-  let adjacent_2_combined:Libcrux_intrinsics.Avx2_extract.t_Vec256 =
+  let adjacent_2_combined:u8 =
     Libcrux_intrinsics.Avx2_extract.mm256_srli_epi64 14l adjacent_2_combined
   in
-  let every_second_element:Libcrux_intrinsics.Avx2_extract.t_Vec256 =
+  let every_second_element:u8 =
     Libcrux_intrinsics.Avx2_extract.mm256_bsrli_epi128 8l adjacent_2_combined
   in
-  let every_second_element_shifted:Libcrux_intrinsics.Avx2_extract.t_Vec256 =
+  let every_second_element_shifted:u8 =
     Libcrux_intrinsics.Avx2_extract.mm256_slli_epi64 36l every_second_element
   in
-  let adjacent_4_combined:Libcrux_intrinsics.Avx2_extract.t_Vec256 =
+  let adjacent_4_combined:u8 =
     Libcrux_intrinsics.Avx2_extract.mm256_add_epi64 adjacent_2_combined every_second_element_shifted
   in
-  let adjacent_4_combined:Libcrux_intrinsics.Avx2_extract.t_Vec256 =
+  let adjacent_4_combined:u8 =
     Libcrux_intrinsics.Avx2_extract.mm256_srlv_epi64 adjacent_4_combined
-      (Libcrux_intrinsics.Avx2_extract.mm256_set_epi64x 28L 0L 28L 0L
-        <:
-        Libcrux_intrinsics.Avx2_extract.t_Vec256)
+      (Libcrux_intrinsics.Avx2_extract.mm256_set_epi64x 28L 0L 28L 0L <: u8)
   in
-  let lower_4_:Libcrux_intrinsics.Avx2_extract.t_Vec128 =
-    Libcrux_intrinsics.Avx2_extract.mm256_castsi256_si128 adjacent_4_combined
-  in
+  let lower_4_:u8 = Libcrux_intrinsics.Avx2_extract.mm256_castsi256_si128 adjacent_4_combined in
   let serialized:t_Array u8 (sz 32) =
     Rust_primitives.Hax.Monomorphized_update_at.update_at_range serialized
       ({ Core.Ops.Range.f_start = sz 0; Core.Ops.Range.f_end = sz 16 }
@@ -185,7 +172,7 @@ let serialize_when_gamma1_is_2_pow_17_
         <:
         t_Slice u8)
   in
-  let upper_4_:Libcrux_intrinsics.Avx2_extract.t_Vec128 =
+  let upper_4_:u8 =
     Libcrux_intrinsics.Avx2_extract.mm256_extracti128_si256 1l adjacent_4_combined
   in
   let serialized:t_Array u8 (sz 32) =
@@ -218,38 +205,31 @@ let serialize_when_gamma1_is_2_pow_17_
       <:
       Core.Result.t_Result (t_Array u8 v_OUTPUT_SIZE) Core.Array.t_TryFromSliceError)
 
-let serialize_when_gamma1_is_2_pow_19_
-      (v_OUTPUT_SIZE: usize)
-      (simd_unit: Libcrux_intrinsics.Avx2_extract.t_Vec256)
-     =
+let serialize_when_gamma1_is_2_pow_19_ (v_OUTPUT_SIZE: usize) (simd_unit: u8) =
   let serialized:t_Array u8 (sz 32) = Rust_primitives.Hax.repeat 0uy (sz 32) in
-  let simd_unit_shifted:Libcrux_intrinsics.Avx2_extract.t_Vec256 =
+  let simd_unit_shifted:u8 =
     Libcrux_intrinsics.Avx2_extract.mm256_sub_epi32 (Libcrux_intrinsics.Avx2_extract.mm256_set1_epi32
           serialize_when_gamma1_is_2_pow_19___GAMMA1
         <:
-        Libcrux_intrinsics.Avx2_extract.t_Vec256)
+        u8)
       simd_unit
   in
-  let adjacent_2_combined:Libcrux_intrinsics.Avx2_extract.t_Vec256 =
+  let adjacent_2_combined:u8 =
     Libcrux_intrinsics.Avx2_extract.mm256_sllv_epi32 simd_unit_shifted
-      (Libcrux_intrinsics.Avx2_extract.mm256_set_epi32 0l 12l 0l 12l 0l 12l 0l 12l
-        <:
-        Libcrux_intrinsics.Avx2_extract.t_Vec256)
+      (Libcrux_intrinsics.Avx2_extract.mm256_set_epi32 0l 12l 0l 12l 0l 12l 0l 12l <: u8)
   in
-  let adjacent_2_combined:Libcrux_intrinsics.Avx2_extract.t_Vec256 =
+  let adjacent_2_combined:u8 =
     Libcrux_intrinsics.Avx2_extract.mm256_srli_epi64 12l adjacent_2_combined
   in
-  let adjacent_4_combined:Libcrux_intrinsics.Avx2_extract.t_Vec256 =
+  let adjacent_4_combined:u8 =
     Libcrux_intrinsics.Avx2_extract.mm256_shuffle_epi8 adjacent_2_combined
       (Libcrux_intrinsics.Avx2_extract.mm256_set_epi8 (-1y) (-1y) (-1y) (-1y) (-1y) (-1y) 12y 11y
           10y 9y 8y 4y 3y 2y 1y 0y (-1y) (-1y) (-1y) (-1y) (-1y) (-1y) 12y 11y 10y 9y 8y 4y 3y 2y 1y
           0y
         <:
-        Libcrux_intrinsics.Avx2_extract.t_Vec256)
+        u8)
   in
-  let lower_4_:Libcrux_intrinsics.Avx2_extract.t_Vec128 =
-    Libcrux_intrinsics.Avx2_extract.mm256_castsi256_si128 adjacent_4_combined
-  in
+  let lower_4_:u8 = Libcrux_intrinsics.Avx2_extract.mm256_castsi256_si128 adjacent_4_combined in
   let serialized:t_Array u8 (sz 32) =
     Rust_primitives.Hax.Monomorphized_update_at.update_at_range serialized
       ({ Core.Ops.Range.f_start = sz 0; Core.Ops.Range.f_end = sz 16 }
@@ -267,7 +247,7 @@ let serialize_when_gamma1_is_2_pow_19_
         <:
         t_Slice u8)
   in
-  let upper_4_:Libcrux_intrinsics.Avx2_extract.t_Vec128 =
+  let upper_4_:u8 =
     Libcrux_intrinsics.Avx2_extract.mm256_extracti128_si256 1l adjacent_4_combined
   in
   let serialized:t_Array u8 (sz 32) =
@@ -300,7 +280,7 @@ let serialize_when_gamma1_is_2_pow_19_
       <:
       Core.Result.t_Result (t_Array u8 v_OUTPUT_SIZE) Core.Array.t_TryFromSliceError)
 
-let serialize (v_OUTPUT_SIZE: usize) (simd_unit: Libcrux_intrinsics.Avx2_extract.t_Vec256) =
+let serialize (v_OUTPUT_SIZE: usize) (simd_unit: u8) =
   match cast (v_OUTPUT_SIZE <: usize) <: u8 with
   | 18uy -> serialize_when_gamma1_is_2_pow_17_ v_OUTPUT_SIZE simd_unit
   | 20uy -> serialize_when_gamma1_is_2_pow_19_ v_OUTPUT_SIZE simd_unit
