libcrux-ml-dsa/proofs/fstar/extraction/Libcrux_ml_dsa.Simd.Avx2.Arithmetic.fst
@@ -3,30 +3,27 @@ module Libcrux_ml_dsa.Simd.Avx2.Arithmetic
 open Core
 open FStar.Mul
 
-let add (lhs rhs: Libcrux_intrinsics.Avx2_extract.t_Vec256) =
-  Libcrux_intrinsics.Avx2_extract.mm256_add_epi32 lhs rhs
+let add (lhs rhs: u8) = Libcrux_intrinsics.Avx2_extract.mm256_add_epi32 lhs rhs
 
-let compute_hint (v_GAMMA2: i32) (low high: Libcrux_intrinsics.Avx2_extract.t_Vec256) =
-  let gamma2:Libcrux_intrinsics.Avx2_extract.t_Vec256 =
-    Libcrux_intrinsics.Avx2_extract.mm256_set1_epi32 v_GAMMA2
-  in
-  let minus_gamma2:Libcrux_intrinsics.Avx2_extract.t_Vec256 =
+let compute_hint (v_GAMMA2: i32) (low high: u8) =
+  let gamma2:u8 = Libcrux_intrinsics.Avx2_extract.mm256_set1_epi32 v_GAMMA2 in
+  let minus_gamma2:u8 =
     Libcrux_intrinsics.Avx2_extract.mm256_set1_epi32 (Core.Ops.Arith.Neg.neg v_GAMMA2 <: i32)
   in
-  let low_within_bound:Libcrux_intrinsics.Avx2_extract.t_Vec256 =
+  let low_within_bound:u8 =
     Libcrux_intrinsics.Avx2_extract.mm256_cmpgt_epi32 (Libcrux_intrinsics.Avx2_extract.mm256_abs_epi32
           low
         <:
-        Libcrux_intrinsics.Avx2_extract.t_Vec256)
+        u8)
       gamma2
   in
-  let low_equals_minus_gamma2:Libcrux_intrinsics.Avx2_extract.t_Vec256 =
+  let low_equals_minus_gamma2:u8 =
     Libcrux_intrinsics.Avx2_extract.mm256_cmpeq_epi32 low minus_gamma2
   in
-  let low_equals_minus_gamma2_and_high_is_nonzero:Libcrux_intrinsics.Avx2_extract.t_Vec256 =
+  let low_equals_minus_gamma2_and_high_is_nonzero:u8 =
     Libcrux_intrinsics.Avx2_extract.mm256_sign_epi32 low_equals_minus_gamma2 high
   in
-  let hints:Libcrux_intrinsics.Avx2_extract.t_Vec256 =
+  let hints:u8 =
     Libcrux_intrinsics.Avx2_extract.mm256_or_si256 low_within_bound
       low_equals_minus_gamma2_and_high_is_nonzero
   in
@@ -38,19 +35,14 @@ let compute_hint (v_GAMMA2: i32) (low high: Libcrux_intrinsics.Avx2_extract.t_Ve
   in
   (cast (Core.Num.impl__i32__count_ones hints_mask <: u32) <: usize),
   Libcrux_intrinsics.Avx2_extract.mm256_and_si256 hints
-    (Libcrux_intrinsics.Avx2_extract.mm256_set1_epi32 1l <: Libcrux_intrinsics.Avx2_extract.t_Vec256
-    )
+    (Libcrux_intrinsics.Avx2_extract.mm256_set1_epi32 1l <: u8)
   <:
-  (usize & Libcrux_intrinsics.Avx2_extract.t_Vec256)
+  (usize & u8)
 
-let infinity_norm_exceeds (simd_unit: Libcrux_intrinsics.Avx2_extract.t_Vec256) (bound: i32) =
-  let absolute_values:Libcrux_intrinsics.Avx2_extract.t_Vec256 =
-    Libcrux_intrinsics.Avx2_extract.mm256_abs_epi32 simd_unit
-  in
-  let bound:Libcrux_intrinsics.Avx2_extract.t_Vec256 =
-    Libcrux_intrinsics.Avx2_extract.mm256_set1_epi32 (bound -! 1l <: i32)
-  in
-  let compare_with_bound:Libcrux_intrinsics.Avx2_extract.t_Vec256 =
+let infinity_norm_exceeds (simd_unit: u8) (bound: i32) =
+  let absolute_values:u8 = Libcrux_intrinsics.Avx2_extract.mm256_abs_epi32 simd_unit in
+  let bound:u8 = Libcrux_intrinsics.Avx2_extract.mm256_set1_epi32 (bound -! 1l <: i32) in
+  let compare_with_bound:u8 =
     Libcrux_intrinsics.Avx2_extract.mm256_cmpgt_epi32 absolute_values bound
   in
   let result:i32 =
@@ -58,45 +50,36 @@ let infinity_norm_exceeds (simd_unit: Libcrux_intrinsics.Avx2_extract.t_Vec256) 
   in
   if result =. 1l then false else true
 
-let subtract (lhs rhs: Libcrux_intrinsics.Avx2_extract.t_Vec256) =
-  Libcrux_intrinsics.Avx2_extract.mm256_sub_epi32 lhs rhs
+let subtract (lhs rhs: u8) = Libcrux_intrinsics.Avx2_extract.mm256_sub_epi32 lhs rhs
 
-let shift_left_then_reduce (v_SHIFT_BY: i32) (simd_unit: Libcrux_intrinsics.Avx2_extract.t_Vec256) =
-  let shifted:Libcrux_intrinsics.Avx2_extract.t_Vec256 =
-    Libcrux_intrinsics.Avx2_extract.mm256_slli_epi32 v_SHIFT_BY simd_unit
-  in
-  let quotient:Libcrux_intrinsics.Avx2_extract.t_Vec256 =
+let shift_left_then_reduce (v_SHIFT_BY: i32) (simd_unit: u8) =
+  let shifted:u8 = Libcrux_intrinsics.Avx2_extract.mm256_slli_epi32 v_SHIFT_BY simd_unit in
+  let quotient:u8 =
     Libcrux_intrinsics.Avx2_extract.mm256_add_epi32 shifted
-      (Libcrux_intrinsics.Avx2_extract.mm256_set1_epi32 (1l <<! 22l <: i32)
-        <:
-        Libcrux_intrinsics.Avx2_extract.t_Vec256)
+      (Libcrux_intrinsics.Avx2_extract.mm256_set1_epi32 (1l <<! 22l <: i32) <: u8)
   in
-  let quotient:Libcrux_intrinsics.Avx2_extract.t_Vec256 =
-    Libcrux_intrinsics.Avx2_extract.mm256_srai_epi32 23l quotient
-  in
-  let quotient_times_field_modulus:Libcrux_intrinsics.Avx2_extract.t_Vec256 =
+  let quotient:u8 = Libcrux_intrinsics.Avx2_extract.mm256_srai_epi32 23l quotient in
+  let quotient_times_field_modulus:u8 =
     Libcrux_intrinsics.Avx2_extract.mm256_mullo_epi32 quotient
       (Libcrux_intrinsics.Avx2_extract.mm256_set1_epi32 Libcrux_ml_dsa.Simd.Traits.v_FIELD_MODULUS
         <:
-        Libcrux_intrinsics.Avx2_extract.t_Vec256)
+        u8)
   in
   Libcrux_intrinsics.Avx2_extract.mm256_sub_epi32 shifted quotient_times_field_modulus
 
-let to_unsigned_representatives (t: Libcrux_intrinsics.Avx2_extract.t_Vec256) =
-  let signs:Libcrux_intrinsics.Avx2_extract.t_Vec256 =
-    Libcrux_intrinsics.Avx2_extract.mm256_srai_epi32 31l t
-  in
-  let conditional_add_field_modulus:Libcrux_intrinsics.Avx2_extract.t_Vec256 =
+let to_unsigned_representatives (t: u8) =
+  let signs:u8 = Libcrux_intrinsics.Avx2_extract.mm256_srai_epi32 31l t in
+  let conditional_add_field_modulus:u8 =
     Libcrux_intrinsics.Avx2_extract.mm256_and_si256 signs
       (Libcrux_intrinsics.Avx2_extract.mm256_set1_epi32 Libcrux_ml_dsa.Simd.Traits.v_FIELD_MODULUS
         <:
-        Libcrux_intrinsics.Avx2_extract.t_Vec256)
+        u8)
   in
   Libcrux_intrinsics.Avx2_extract.mm256_add_epi32 t conditional_add_field_modulus
 
-let power2round (r: Libcrux_intrinsics.Avx2_extract.t_Vec256) =
-  let r:Libcrux_intrinsics.Avx2_extract.t_Vec256 = to_unsigned_representatives r in
-  let r1:Libcrux_intrinsics.Avx2_extract.t_Vec256 =
+let power2round (r: u8) =
+  let r:u8 = to_unsigned_representatives r in
+  let r1:u8 =
     Libcrux_intrinsics.Avx2_extract.mm256_add_epi32 r
       (Libcrux_intrinsics.Avx2_extract.mm256_set1_epi32 ((1l <<!
               (Libcrux_ml_dsa.Constants.v_BITS_IN_LOWER_PART_OF_T -! sz 1 <: usize)
@@ -106,119 +89,83 @@ let power2round (r: Libcrux_intrinsics.Avx2_extract.t_Vec256) =
             <:
             i32)
         <:
-        Libcrux_intrinsics.Avx2_extract.t_Vec256)
+        u8)
   in
-  let r1:Libcrux_intrinsics.Avx2_extract.t_Vec256 =
-    Libcrux_intrinsics.Avx2_extract.mm256_srai_epi32 13l r1
-  in
-  let r0:Libcrux_intrinsics.Avx2_extract.t_Vec256 =
-    Libcrux_intrinsics.Avx2_extract.mm256_slli_epi32 13l r1
-  in
-  let r0:Libcrux_intrinsics.Avx2_extract.t_Vec256 =
-    Libcrux_intrinsics.Avx2_extract.mm256_sub_epi32 r r0
-  in
-  r0, r1 <: (Libcrux_intrinsics.Avx2_extract.t_Vec256 & Libcrux_intrinsics.Avx2_extract.t_Vec256)
+  let r1:u8 = Libcrux_intrinsics.Avx2_extract.mm256_srai_epi32 13l r1 in
+  let r0:u8 = Libcrux_intrinsics.Avx2_extract.mm256_slli_epi32 13l r1 in
+  let r0:u8 = Libcrux_intrinsics.Avx2_extract.mm256_sub_epi32 r r0 in
+  r0, r1 <: (u8 & u8)
 
-let montgomery_multiply (lhs rhs: Libcrux_intrinsics.Avx2_extract.t_Vec256) =
-  let field_modulus:Libcrux_intrinsics.Avx2_extract.t_Vec256 =
+let montgomery_multiply (lhs rhs: u8) =
+  let field_modulus:u8 =
     Libcrux_intrinsics.Avx2_extract.mm256_set1_epi32 Libcrux_ml_dsa.Simd.Traits.v_FIELD_MODULUS
   in
-  let inverse_of_modulus_mod_montgomery_r:Libcrux_intrinsics.Avx2_extract.t_Vec256 =
+  let inverse_of_modulus_mod_montgomery_r:u8 =
     Libcrux_intrinsics.Avx2_extract.mm256_set1_epi32 (cast (Libcrux_ml_dsa.Simd.Traits.v_INVERSE_OF_MODULUS_MOD_MONTGOMERY_R
             <:
             u64)
         <:
         i32)
   in
-  let prod02:Libcrux_intrinsics.Avx2_extract.t_Vec256 =
-    Libcrux_intrinsics.Avx2_extract.mm256_mul_epi32 lhs rhs
-  in
-  let prod13:Libcrux_intrinsics.Avx2_extract.t_Vec256 =
+  let prod02:u8 = Libcrux_intrinsics.Avx2_extract.mm256_mul_epi32 lhs rhs in
+  let prod13:u8 =
     Libcrux_intrinsics.Avx2_extract.mm256_mul_epi32 (Libcrux_intrinsics.Avx2_extract.mm256_shuffle_epi32
           245l
           lhs
         <:
-        Libcrux_intrinsics.Avx2_extract.t_Vec256)
-      (Libcrux_intrinsics.Avx2_extract.mm256_shuffle_epi32 245l rhs
-        <:
-        Libcrux_intrinsics.Avx2_extract.t_Vec256)
+        u8)
+      (Libcrux_intrinsics.Avx2_extract.mm256_shuffle_epi32 245l rhs <: u8)
   in
-  let k02:Libcrux_intrinsics.Avx2_extract.t_Vec256 =
+  let k02:u8 =
     Libcrux_intrinsics.Avx2_extract.mm256_mul_epi32 prod02 inverse_of_modulus_mod_montgomery_r
   in
-  let k13:Libcrux_intrinsics.Avx2_extract.t_Vec256 =
+  let k13:u8 =
     Libcrux_intrinsics.Avx2_extract.mm256_mul_epi32 prod13 inverse_of_modulus_mod_montgomery_r
   in
-  let c02:Libcrux_intrinsics.Avx2_extract.t_Vec256 =
-    Libcrux_intrinsics.Avx2_extract.mm256_mul_epi32 k02 field_modulus
-  in
-  let c13:Libcrux_intrinsics.Avx2_extract.t_Vec256 =
-    Libcrux_intrinsics.Avx2_extract.mm256_mul_epi32 k13 field_modulus
-  in
-  let res02:Libcrux_intrinsics.Avx2_extract.t_Vec256 =
-    Libcrux_intrinsics.Avx2_extract.mm256_sub_epi32 prod02 c02
-  in
-  let res13:Libcrux_intrinsics.Avx2_extract.t_Vec256 =
-    Libcrux_intrinsics.Avx2_extract.mm256_sub_epi32 prod13 c13
-  in
-  let res02_shifted:Libcrux_intrinsics.Avx2_extract.t_Vec256 =
-    Libcrux_intrinsics.Avx2_extract.mm256_shuffle_epi32 245l res02
-  in
+  let c02:u8 = Libcrux_intrinsics.Avx2_extract.mm256_mul_epi32 k02 field_modulus in
+  let c13:u8 = Libcrux_intrinsics.Avx2_extract.mm256_mul_epi32 k13 field_modulus in
+  let res02:u8 = Libcrux_intrinsics.Avx2_extract.mm256_sub_epi32 prod02 c02 in
+  let res13:u8 = Libcrux_intrinsics.Avx2_extract.mm256_sub_epi32 prod13 c13 in
+  let res02_shifted:u8 = Libcrux_intrinsics.Avx2_extract.mm256_shuffle_epi32 245l res02 in
   Libcrux_intrinsics.Avx2_extract.mm256_blend_epi32 170l res02_shifted res13
 
-let montgomery_multiply_by_constant (lhs: Libcrux_intrinsics.Avx2_extract.t_Vec256) (constant: i32) =
-  let rhs:Libcrux_intrinsics.Avx2_extract.t_Vec256 =
-    Libcrux_intrinsics.Avx2_extract.mm256_set1_epi32 constant
-  in
-  let field_modulus:Libcrux_intrinsics.Avx2_extract.t_Vec256 =
+let montgomery_multiply_by_constant (lhs: u8) (constant: i32) =
+  let rhs:u8 = Libcrux_intrinsics.Avx2_extract.mm256_set1_epi32 constant in
+  let field_modulus:u8 =
     Libcrux_intrinsics.Avx2_extract.mm256_set1_epi32 Libcrux_ml_dsa.Simd.Traits.v_FIELD_MODULUS
   in
-  let inverse_of_modulus_mod_montgomery_r:Libcrux_intrinsics.Avx2_extract.t_Vec256 =
+  let inverse_of_modulus_mod_montgomery_r:u8 =
     Libcrux_intrinsics.Avx2_extract.mm256_set1_epi32 (cast (Libcrux_ml_dsa.Simd.Traits.v_INVERSE_OF_MODULUS_MOD_MONTGOMERY_R
             <:
             u64)
         <:
         i32)
   in
-  let prod02:Libcrux_intrinsics.Avx2_extract.t_Vec256 =
-    Libcrux_intrinsics.Avx2_extract.mm256_mul_epi32 lhs rhs
-  in
-  let prod13:Libcrux_intrinsics.Avx2_extract.t_Vec256 =
+  let prod02:u8 = Libcrux_intrinsics.Avx2_extract.mm256_mul_epi32 lhs rhs in
+  let prod13:u8 =
     Libcrux_intrinsics.Avx2_extract.mm256_mul_epi32 (Libcrux_intrinsics.Avx2_extract.mm256_shuffle_epi32
           245l
           lhs
         <:
-        Libcrux_intrinsics.Avx2_extract.t_Vec256)
-      (Libcrux_intrinsics.Avx2_extract.mm256_shuffle_epi32 245l rhs
-        <:
-        Libcrux_intrinsics.Avx2_extract.t_Vec256)
+        u8)
+      (Libcrux_intrinsics.Avx2_extract.mm256_shuffle_epi32 245l rhs <: u8)
   in
-  let k02:Libcrux_intrinsics.Avx2_extract.t_Vec256 =
+  let k02:u8 =
     Libcrux_intrinsics.Avx2_extract.mm256_mul_epi32 prod02 inverse_of_modulus_mod_montgomery_r
   in
-  let k13:Libcrux_intrinsics.Avx2_extract.t_Vec256 =
+  let k13:u8 =
     Libcrux_intrinsics.Avx2_extract.mm256_mul_epi32 prod13 inverse_of_modulus_mod_montgomery_r
   in
-  let c02:Libcrux_intrinsics.Avx2_extract.t_Vec256 =
-    Libcrux_intrinsics.Avx2_extract.mm256_mul_epi32 k02 field_modulus
-  in
-  let c13:Libcrux_intrinsics.Avx2_extract.t_Vec256 =
-    Libcrux_intrinsics.Avx2_extract.mm256_mul_epi32 k13 field_modulus
-  in
-  let res02:Libcrux_intrinsics.Avx2_extract.t_Vec256 =
-    Libcrux_intrinsics.Avx2_extract.mm256_sub_epi32 prod02 c02
-  in
-  let res13:Libcrux_intrinsics.Avx2_extract.t_Vec256 =
-    Libcrux_intrinsics.Avx2_extract.mm256_sub_epi32 prod13 c13
-  in
-  let res02_shifted:Libcrux_intrinsics.Avx2_extract.t_Vec256 =
-    Libcrux_intrinsics.Avx2_extract.mm256_shuffle_epi32 245l res02
-  in
+  let c02:u8 = Libcrux_intrinsics.Avx2_extract.mm256_mul_epi32 k02 field_modulus in
+  let c13:u8 = Libcrux_intrinsics.Avx2_extract.mm256_mul_epi32 k13 field_modulus in
+  let res02:u8 = Libcrux_intrinsics.Avx2_extract.mm256_sub_epi32 prod02 c02 in
+  let res13:u8 = Libcrux_intrinsics.Avx2_extract.mm256_sub_epi32 prod13 c13 in
+  let res02_shifted:u8 = Libcrux_intrinsics.Avx2_extract.mm256_shuffle_epi32 245l res02 in
   Libcrux_intrinsics.Avx2_extract.mm256_blend_epi32 170l res02_shifted res13
 
-let decompose (v_GAMMA2: i32) (r: Libcrux_intrinsics.Avx2_extract.t_Vec256) =
-  let r:Libcrux_intrinsics.Avx2_extract.t_Vec256 = to_unsigned_representatives r in
-  let field_modulus_halved:Libcrux_intrinsics.Avx2_extract.t_Vec256 =
+let decompose (v_GAMMA2: i32) (r: u8) =
+  let r:u8 = to_unsigned_representatives r in
+  let field_modulus_halved:u8 =
     Libcrux_intrinsics.Avx2_extract.mm256_set1_epi32 ((Libcrux_ml_dsa.Simd.Traits.v_FIELD_MODULUS -!
           1l
           <:
@@ -228,127 +175,83 @@ let decompose (v_GAMMA2: i32) (r: Libcrux_intrinsics.Avx2_extract.t_Vec256) =
         i32)
   in
   let (v_ALPHA: i32):i32 = v_GAMMA2 *! 2l in
-  let ceil_of_r_by_128_:Libcrux_intrinsics.Avx2_extract.t_Vec256 =
+  let ceil_of_r_by_128_:u8 =
     Libcrux_intrinsics.Avx2_extract.mm256_add_epi32 r
-      (Libcrux_intrinsics.Avx2_extract.mm256_set1_epi32 127l
-        <:
-        Libcrux_intrinsics.Avx2_extract.t_Vec256)
+      (Libcrux_intrinsics.Avx2_extract.mm256_set1_epi32 127l <: u8)
   in
-  let ceil_of_r_by_128_:Libcrux_intrinsics.Avx2_extract.t_Vec256 =
+  let ceil_of_r_by_128_:u8 =
     Libcrux_intrinsics.Avx2_extract.mm256_srai_epi32 7l ceil_of_r_by_128_
   in
-  let r1:Libcrux_intrinsics.Avx2_extract.t_Vec256 =
+  let r1:u8 =
     match v_ALPHA with
     | 190464l ->
-      let result:Libcrux_intrinsics.Avx2_extract.t_Vec256 =
+      let result:u8 =
         Libcrux_intrinsics.Avx2_extract.mm256_mullo_epi32 ceil_of_r_by_128_
-          (Libcrux_intrinsics.Avx2_extract.mm256_set1_epi32 11275l
-            <:
-            Libcrux_intrinsics.Avx2_extract.t_Vec256)
+          (Libcrux_intrinsics.Avx2_extract.mm256_set1_epi32 11275l <: u8)
       in
-      let result:Libcrux_intrinsics.Avx2_extract.t_Vec256 =
+      let result:u8 =
         Libcrux_intrinsics.Avx2_extract.mm256_add_epi32 result
-          (Libcrux_intrinsics.Avx2_extract.mm256_set1_epi32 (1l <<! 23l <: i32)
-            <:
-            Libcrux_intrinsics.Avx2_extract.t_Vec256)
+          (Libcrux_intrinsics.Avx2_extract.mm256_set1_epi32 (1l <<! 23l <: i32) <: u8)
       in
-      let result:Libcrux_intrinsics.Avx2_extract.t_Vec256 =
-        Libcrux_intrinsics.Avx2_extract.mm256_srai_epi32 24l result
-      in
-      let mask:Libcrux_intrinsics.Avx2_extract.t_Vec256 =
+      let result:u8 = Libcrux_intrinsics.Avx2_extract.mm256_srai_epi32 24l result in
+      let mask:u8 =
         Libcrux_intrinsics.Avx2_extract.mm256_sub_epi32 (Libcrux_intrinsics.Avx2_extract.mm256_set1_epi32
               43l
             <:
-            Libcrux_intrinsics.Avx2_extract.t_Vec256)
+            u8)
           result
       in
-      let mask:Libcrux_intrinsics.Avx2_extract.t_Vec256 =
-        Libcrux_intrinsics.Avx2_extract.mm256_srai_epi32 31l mask
-      in
-      let not_result:Libcrux_intrinsics.Avx2_extract.t_Vec256 =
-        Libcrux_intrinsics.Avx2_extract.mm256_xor_si256 result mask
-      in
+      let mask:u8 = Libcrux_intrinsics.Avx2_extract.mm256_srai_epi32 31l mask in
+      let not_result:u8 = Libcrux_intrinsics.Avx2_extract.mm256_xor_si256 result mask in
       Libcrux_intrinsics.Avx2_extract.mm256_and_si256 result not_result
     | 523776l ->
-      let result:Libcrux_intrinsics.Avx2_extract.t_Vec256 =
+      let result:u8 =
         Libcrux_intrinsics.Avx2_extract.mm256_mullo_epi32 ceil_of_r_by_128_
-          (Libcrux_intrinsics.Avx2_extract.mm256_set1_epi32 1025l
-            <:
-            Libcrux_intrinsics.Avx2_extract.t_Vec256)
+          (Libcrux_intrinsics.Avx2_extract.mm256_set1_epi32 1025l <: u8)
       in
-      let result:Libcrux_intrinsics.Avx2_extract.t_Vec256 =
+      let result:u8 =
         Libcrux_intrinsics.Avx2_extract.mm256_add_epi32 result
-          (Libcrux_intrinsics.Avx2_extract.mm256_set1_epi32 (1l <<! 21l <: i32)
-            <:
-            Libcrux_intrinsics.Avx2_extract.t_Vec256)
+          (Libcrux_intrinsics.Avx2_extract.mm256_set1_epi32 (1l <<! 21l <: i32) <: u8)
       in
-      let result:Libcrux_intrinsics.Avx2_extract.t_Vec256 =
-        Libcrux_intrinsics.Avx2_extract.mm256_srai_epi32 22l result
-      in
+      let result:u8 = Libcrux_intrinsics.Avx2_extract.mm256_srai_epi32 22l result in
       Libcrux_intrinsics.Avx2_extract.mm256_and_si256 result
-        (Libcrux_intrinsics.Avx2_extract.mm256_set1_epi32 15l
-          <:
-          Libcrux_intrinsics.Avx2_extract.t_Vec256)
+        (Libcrux_intrinsics.Avx2_extract.mm256_set1_epi32 15l <: u8)
     | _ ->
       Rust_primitives.Hax.never_to_any (Core.Panicking.panic "internal error: entered unreachable code"
 
           <:
           Rust_primitives.Hax.t_Never)
   in
-  let r0:Libcrux_intrinsics.Avx2_extract.t_Vec256 =
+  let r0:u8 =
     Libcrux_intrinsics.Avx2_extract.mm256_mullo_epi32 r1
-      (Libcrux_intrinsics.Avx2_extract.mm256_set1_epi32 v_ALPHA
-        <:
-        Libcrux_intrinsics.Avx2_extract.t_Vec256)
+      (Libcrux_intrinsics.Avx2_extract.mm256_set1_epi32 v_ALPHA <: u8)
   in
-  let r0:Libcrux_intrinsics.Avx2_extract.t_Vec256 =
-    Libcrux_intrinsics.Avx2_extract.mm256_sub_epi32 r r0
-  in
-  let mask:Libcrux_intrinsics.Avx2_extract.t_Vec256 =
-    Libcrux_intrinsics.Avx2_extract.mm256_sub_epi32 field_modulus_halved r0
-  in
-  let mask:Libcrux_intrinsics.Avx2_extract.t_Vec256 =
-    Libcrux_intrinsics.Avx2_extract.mm256_srai_epi32 31l mask
-  in
-  let field_modulus_and_mask:Libcrux_intrinsics.Avx2_extract.t_Vec256 =
+  let r0:u8 = Libcrux_intrinsics.Avx2_extract.mm256_sub_epi32 r r0 in
+  let mask:u8 = Libcrux_intrinsics.Avx2_extract.mm256_sub_epi32 field_modulus_halved r0 in
+  let mask:u8 = Libcrux_intrinsics.Avx2_extract.mm256_srai_epi32 31l mask in
+  let field_modulus_and_mask:u8 =
     Libcrux_intrinsics.Avx2_extract.mm256_and_si256 mask
       (Libcrux_intrinsics.Avx2_extract.mm256_set1_epi32 Libcrux_ml_dsa.Simd.Traits.v_FIELD_MODULUS
         <:
-        Libcrux_intrinsics.Avx2_extract.t_Vec256)
+        u8)
   in
-  let r0:Libcrux_intrinsics.Avx2_extract.t_Vec256 =
-    Libcrux_intrinsics.Avx2_extract.mm256_sub_epi32 r0 field_modulus_and_mask
-  in
-  r0, r1 <: (Libcrux_intrinsics.Avx2_extract.t_Vec256 & Libcrux_intrinsics.Avx2_extract.t_Vec256)
+  let r0:u8 = Libcrux_intrinsics.Avx2_extract.mm256_sub_epi32 r0 field_modulus_and_mask in
+  r0, r1 <: (u8 & u8)
 
-let use_hint (v_GAMMA2: i32) (r hint: Libcrux_intrinsics.Avx2_extract.t_Vec256) =
-  let r0, r1:(Libcrux_intrinsics.Avx2_extract.t_Vec256 & Libcrux_intrinsics.Avx2_extract.t_Vec256) =
-    decompose v_GAMMA2 r
-  in
-  let all_zeros:Libcrux_intrinsics.Avx2_extract.t_Vec256 =
-    Libcrux_intrinsics.Avx2_extract.mm256_setzero_si256 ()
-  in
-  let negate_hints:Libcrux_intrinsics.Avx2_extract.t_Vec256 =
-    Libcrux_intrinsics.Avx2_extract.vec256_blendv_epi32 all_zeros hint r0
-  in
-  let negate_hints:Libcrux_intrinsics.Avx2_extract.t_Vec256 =
-    Libcrux_intrinsics.Avx2_extract.mm256_slli_epi32 1l negate_hints
-  in
-  let hints:Libcrux_intrinsics.Avx2_extract.t_Vec256 =
-    Libcrux_intrinsics.Avx2_extract.mm256_sub_epi32 hint negate_hints
-  in
-  let r1_plus_hints:Libcrux_intrinsics.Avx2_extract.t_Vec256 =
-    Libcrux_intrinsics.Avx2_extract.mm256_add_epi32 r1 hints
-  in
+let use_hint (v_GAMMA2: i32) (r hint: u8) =
+  let r0, r1:(u8 & u8) = decompose v_GAMMA2 r in
+  let all_zeros:u8 = Libcrux_intrinsics.Avx2_extract.mm256_setzero_si256 () in
+  let negate_hints:u8 = Libcrux_intrinsics.Avx2_extract.vec256_blendv_epi32 all_zeros hint r0 in
+  let negate_hints:u8 = Libcrux_intrinsics.Avx2_extract.mm256_slli_epi32 1l negate_hints in
+  let hints:u8 = Libcrux_intrinsics.Avx2_extract.mm256_sub_epi32 hint negate_hints in
+  let r1_plus_hints:u8 = Libcrux_intrinsics.Avx2_extract.mm256_add_epi32 r1 hints in
   match v_GAMMA2 with
   | 95232l ->
-    let max:Libcrux_intrinsics.Avx2_extract.t_Vec256 =
-      Libcrux_intrinsics.Avx2_extract.mm256_set1_epi32 43l
-    in
-    let r1_plus_hints:Libcrux_intrinsics.Avx2_extract.t_Vec256 =
+    let max:u8 = Libcrux_intrinsics.Avx2_extract.mm256_set1_epi32 43l in
+    let r1_plus_hints:u8 =
       Libcrux_intrinsics.Avx2_extract.vec256_blendv_epi32 r1_plus_hints max r1_plus_hints
     in
-    let greater_than_or_equal_to_max:Libcrux_intrinsics.Avx2_extract.t_Vec256 =
+    let greater_than_or_equal_to_max:u8 =
       Libcrux_intrinsics.Avx2_extract.mm256_cmpgt_epi32 r1_plus_hints max
     in
     Libcrux_intrinsics.Avx2_extract.vec256_blendv_epi32 r1_plus_hints
@@ -356,9 +259,7 @@ let use_hint (v_GAMMA2: i32) (r hint: Libcrux_intrinsics.Avx2_extract.t_Vec256) 
       greater_than_or_equal_to_max
   | 261888l ->
     Libcrux_intrinsics.Avx2_extract.mm256_and_si256 r1_plus_hints
-      (Libcrux_intrinsics.Avx2_extract.mm256_set1_epi32 15l
-        <:
-        Libcrux_intrinsics.Avx2_extract.t_Vec256)
+      (Libcrux_intrinsics.Avx2_extract.mm256_set1_epi32 15l <: u8)
   | _ ->
     Rust_primitives.Hax.never_to_any (Core.Panicking.panic "internal error: entered unreachable code"
 
