libcrux-ml-dsa/proofs/fstar/extraction/Libcrux_ml_dsa.Simd.Avx2.Encoding.T1.fsti
@@ -5,8 +5,6 @@ open FStar.Mul
 
 let deserialize__COEFFICIENT_MASK: i32 = (1l <<! 10l <: i32) -! 1l
 
-val serialize (simd_unit: Libcrux_intrinsics.Avx2_extract.t_Vec256)
-    : Prims.Pure (t_Array u8 (sz 10)) Prims.l_True (fun _ -> Prims.l_True)
+val serialize (simd_unit: u8) : Prims.Pure (t_Array u8 (sz 10)) Prims.l_True (fun _ -> Prims.l_True)
 
-val deserialize (bytes: t_Slice u8)
-    : Prims.Pure Libcrux_intrinsics.Avx2_extract.t_Vec256 Prims.l_True (fun _ -> Prims.l_True)
+val deserialize (bytes: t_Slice u8) : Prims.Pure u8 Prims.l_True (fun _ -> Prims.l_True)
