libcrux-ml-dsa/proofs/fstar/extraction/Libcrux_ml_dsa.Simd.Avx2.Ntt.fst
@@ -3,23 +3,14 @@ module Libcrux_ml_dsa.Simd.Avx2.Ntt
 open Core
 open FStar.Mul
 
-let butterfly_2_
-      (a b: Libcrux_intrinsics.Avx2_extract.t_Vec256)
-      (zeta_a0 zeta_a1 zeta_a2 zeta_a3 zeta_b0 zeta_b1 zeta_b2 zeta_b3: i32)
-     =
-  let a_shuffled:Libcrux_intrinsics.Avx2_extract.t_Vec256 =
-    Libcrux_intrinsics.Avx2_extract.mm256_shuffle_epi32 216l a
-  in
-  let b_shuffled:Libcrux_intrinsics.Avx2_extract.t_Vec256 =
-    Libcrux_intrinsics.Avx2_extract.mm256_shuffle_epi32 216l b
-  in
-  let summands:Libcrux_intrinsics.Avx2_extract.t_Vec256 =
-    Libcrux_intrinsics.Avx2_extract.mm256_unpacklo_epi64 a_shuffled b_shuffled
-  in
-  let zeta_multiplicands:Libcrux_intrinsics.Avx2_extract.t_Vec256 =
+let butterfly_2_ (a b: u8) (zeta_a0 zeta_a1 zeta_a2 zeta_a3 zeta_b0 zeta_b1 zeta_b2 zeta_b3: i32) =
+  let a_shuffled:u8 = Libcrux_intrinsics.Avx2_extract.mm256_shuffle_epi32 216l a in
+  let b_shuffled:u8 = Libcrux_intrinsics.Avx2_extract.mm256_shuffle_epi32 216l b in
+  let summands:u8 = Libcrux_intrinsics.Avx2_extract.mm256_unpacklo_epi64 a_shuffled b_shuffled in
+  let zeta_multiplicands:u8 =
     Libcrux_intrinsics.Avx2_extract.mm256_unpackhi_epi64 a_shuffled b_shuffled
   in
-  let zetas:Libcrux_intrinsics.Avx2_extract.t_Vec256 =
+  let zetas:u8 =
     Libcrux_intrinsics.Avx2_extract.mm256_set_epi32 zeta_b3
       zeta_b2
       zeta_a3
@@ -29,42 +20,25 @@ let butterfly_2_
       zeta_a1
       zeta_a0
   in
-  let zeta_products:Libcrux_intrinsics.Avx2_extract.t_Vec256 =
+  let zeta_products:u8 =
     Libcrux_ml_dsa.Simd.Avx2.Arithmetic.montgomery_multiply zeta_multiplicands zetas
   in
-  let add_terms:Libcrux_intrinsics.Avx2_extract.t_Vec256 =
-    Libcrux_ml_dsa.Simd.Avx2.Arithmetic.add summands zeta_products
-  in
-  let sub_terms:Libcrux_intrinsics.Avx2_extract.t_Vec256 =
-    Libcrux_ml_dsa.Simd.Avx2.Arithmetic.subtract summands zeta_products
-  in
-  let a_terms_shuffled:Libcrux_intrinsics.Avx2_extract.t_Vec256 =
+  let add_terms:u8 = Libcrux_ml_dsa.Simd.Avx2.Arithmetic.add summands zeta_products in
+  let sub_terms:u8 = Libcrux_ml_dsa.Simd.Avx2.Arithmetic.subtract summands zeta_products in
+  let a_terms_shuffled:u8 =
     Libcrux_intrinsics.Avx2_extract.mm256_unpacklo_epi64 add_terms sub_terms
   in
-  let b_terms_shuffled:Libcrux_intrinsics.Avx2_extract.t_Vec256 =
+  let b_terms_shuffled:u8 =
     Libcrux_intrinsics.Avx2_extract.mm256_unpackhi_epi64 add_terms sub_terms
   in
-  let a_out:Libcrux_intrinsics.Avx2_extract.t_Vec256 =
-    Libcrux_intrinsics.Avx2_extract.mm256_shuffle_epi32 216l a_terms_shuffled
-  in
-  let b_out:Libcrux_intrinsics.Avx2_extract.t_Vec256 =
-    Libcrux_intrinsics.Avx2_extract.mm256_shuffle_epi32 216l b_terms_shuffled
-  in
-  a_out, b_out
-  <:
-  (Libcrux_intrinsics.Avx2_extract.t_Vec256 & Libcrux_intrinsics.Avx2_extract.t_Vec256)
+  let a_out:u8 = Libcrux_intrinsics.Avx2_extract.mm256_shuffle_epi32 216l a_terms_shuffled in
+  let b_out:u8 = Libcrux_intrinsics.Avx2_extract.mm256_shuffle_epi32 216l b_terms_shuffled in
+  a_out, b_out <: (u8 & u8)
 
-let butterfly_4_
-      (a b: Libcrux_intrinsics.Avx2_extract.t_Vec256)
-      (zeta_a0 zeta_a1 zeta_b0 zeta_b1: i32)
-     =
-  let summands:Libcrux_intrinsics.Avx2_extract.t_Vec256 =
-    Libcrux_intrinsics.Avx2_extract.mm256_unpacklo_epi64 a b
-  in
-  let zeta_multiplicands:Libcrux_intrinsics.Avx2_extract.t_Vec256 =
-    Libcrux_intrinsics.Avx2_extract.mm256_unpackhi_epi64 a b
-  in
-  let zetas:Libcrux_intrinsics.Avx2_extract.t_Vec256 =
+let butterfly_4_ (a b: u8) (zeta_a0 zeta_a1 zeta_b0 zeta_b1: i32) =
+  let summands:u8 = Libcrux_intrinsics.Avx2_extract.mm256_unpacklo_epi64 a b in
+  let zeta_multiplicands:u8 = Libcrux_intrinsics.Avx2_extract.mm256_unpackhi_epi64 a b in
+  let zetas:u8 =
     Libcrux_intrinsics.Avx2_extract.mm256_set_epi32 zeta_b1
       zeta_b1
       zeta_a1
@@ -74,151 +48,91 @@ let butterfly_4_
       zeta_a0
       zeta_a0
   in
-  let zeta_products:Libcrux_intrinsics.Avx2_extract.t_Vec256 =
+  let zeta_products:u8 =
     Libcrux_ml_dsa.Simd.Avx2.Arithmetic.montgomery_multiply zeta_multiplicands zetas
   in
-  let add_terms:Libcrux_intrinsics.Avx2_extract.t_Vec256 =
-    Libcrux_ml_dsa.Simd.Avx2.Arithmetic.add summands zeta_products
-  in
-  let sub_terms:Libcrux_intrinsics.Avx2_extract.t_Vec256 =
-    Libcrux_ml_dsa.Simd.Avx2.Arithmetic.subtract summands zeta_products
-  in
-  let a_out:Libcrux_intrinsics.Avx2_extract.t_Vec256 =
-    Libcrux_intrinsics.Avx2_extract.mm256_unpacklo_epi64 add_terms sub_terms
-  in
-  let b_out:Libcrux_intrinsics.Avx2_extract.t_Vec256 =
-    Libcrux_intrinsics.Avx2_extract.mm256_unpackhi_epi64 add_terms sub_terms
-  in
-  a_out, b_out
-  <:
-  (Libcrux_intrinsics.Avx2_extract.t_Vec256 & Libcrux_intrinsics.Avx2_extract.t_Vec256)
+  let add_terms:u8 = Libcrux_ml_dsa.Simd.Avx2.Arithmetic.add summands zeta_products in
+  let sub_terms:u8 = Libcrux_ml_dsa.Simd.Avx2.Arithmetic.subtract summands zeta_products in
+  let a_out:u8 = Libcrux_intrinsics.Avx2_extract.mm256_unpacklo_epi64 add_terms sub_terms in
+  let b_out:u8 = Libcrux_intrinsics.Avx2_extract.mm256_unpackhi_epi64 add_terms sub_terms in
+  a_out, b_out <: (u8 & u8)
 
-let butterfly_8_ (a b: Libcrux_intrinsics.Avx2_extract.t_Vec256) (zeta0 zeta1: i32) =
-  let summands:Libcrux_intrinsics.Avx2_extract.t_Vec256 =
+let butterfly_8_ (a b: u8) (zeta0 zeta1: i32) =
+  let summands:u8 =
     Libcrux_intrinsics.Avx2_extract.mm256_set_m128i (Libcrux_intrinsics.Avx2_extract.mm256_castsi256_si128
           b
         <:
-        Libcrux_intrinsics.Avx2_extract.t_Vec128)
-      (Libcrux_intrinsics.Avx2_extract.mm256_castsi256_si128 a
-        <:
-        Libcrux_intrinsics.Avx2_extract.t_Vec128)
+        u8)
+      (Libcrux_intrinsics.Avx2_extract.mm256_castsi256_si128 a <: u8)
   in
-  let zeta_multiplicands:Libcrux_intrinsics.Avx2_extract.t_Vec256 =
-    Libcrux_intrinsics.Avx2_extract.mm256_permute2x128_si256 19l b a
-  in
-  let zetas:Libcrux_intrinsics.Avx2_extract.t_Vec256 =
+  let zeta_multiplicands:u8 = Libcrux_intrinsics.Avx2_extract.mm256_permute2x128_si256 19l b a in
+  let zetas:u8 =
     Libcrux_intrinsics.Avx2_extract.mm256_set_epi32 zeta1 zeta1 zeta1 zeta1 zeta0 zeta0 zeta0 zeta0
   in
-  let zeta_products:Libcrux_intrinsics.Avx2_extract.t_Vec256 =
+  let zeta_products:u8 =
     Libcrux_ml_dsa.Simd.Avx2.Arithmetic.montgomery_multiply zeta_multiplicands zetas
   in
-  let add_terms:Libcrux_intrinsics.Avx2_extract.t_Vec256 =
-    Libcrux_ml_dsa.Simd.Avx2.Arithmetic.add summands zeta_products
-  in
-  let sub_terms:Libcrux_intrinsics.Avx2_extract.t_Vec256 =
-    Libcrux_ml_dsa.Simd.Avx2.Arithmetic.subtract summands zeta_products
-  in
-  let a_out:Libcrux_intrinsics.Avx2_extract.t_Vec256 =
+  let add_terms:u8 = Libcrux_ml_dsa.Simd.Avx2.Arithmetic.add summands zeta_products in
+  let sub_terms:u8 = Libcrux_ml_dsa.Simd.Avx2.Arithmetic.subtract summands zeta_products in
+  let a_out:u8 =
     Libcrux_intrinsics.Avx2_extract.mm256_set_m128i (Libcrux_intrinsics.Avx2_extract.mm256_castsi256_si128
           sub_terms
         <:
-        Libcrux_intrinsics.Avx2_extract.t_Vec128)
-      (Libcrux_intrinsics.Avx2_extract.mm256_castsi256_si128 add_terms
-        <:
-        Libcrux_intrinsics.Avx2_extract.t_Vec128)
+        u8)
+      (Libcrux_intrinsics.Avx2_extract.mm256_castsi256_si128 add_terms <: u8)
   in
-  let b_out:Libcrux_intrinsics.Avx2_extract.t_Vec256 =
-    Libcrux_intrinsics.Avx2_extract.mm256_permute2x128_si256 19l sub_terms add_terms
-  in
-  a_out, b_out
-  <:
-  (Libcrux_intrinsics.Avx2_extract.t_Vec256 & Libcrux_intrinsics.Avx2_extract.t_Vec256)
+  let b_out:u8 = Libcrux_intrinsics.Avx2_extract.mm256_permute2x128_si256 19l sub_terms add_terms in
+  a_out, b_out <: (u8 & u8)
 
-let invert_ntt_at_layer_0_
-      (simd_unit: Libcrux_intrinsics.Avx2_extract.t_Vec256)
-      (zeta0 zeta1 zeta2 zeta3: i32)
-     =
-  let zetas:Libcrux_intrinsics.Avx2_extract.t_Vec256 =
+let invert_ntt_at_layer_0_ (simd_unit: u8) (zeta0 zeta1 zeta2 zeta3: i32) =
+  let zetas:u8 =
     Libcrux_intrinsics.Avx2_extract.mm256_set_epi32 zeta3 0l zeta2 0l zeta1 0l zeta0 0l
   in
-  let add_by_signs:Libcrux_intrinsics.Avx2_extract.t_Vec256 =
+  let add_by_signs:u8 =
     Libcrux_intrinsics.Avx2_extract.mm256_set_epi32 (-1l) 1l (-1l) 1l (-1l) 1l (-1l) 1l
   in
-  let add_by:Libcrux_intrinsics.Avx2_extract.t_Vec256 =
-    Libcrux_intrinsics.Avx2_extract.mm256_shuffle_epi32 177l simd_unit
-  in
-  let add_by:Libcrux_intrinsics.Avx2_extract.t_Vec256 =
-    Libcrux_intrinsics.Avx2_extract.mm256_mullo_epi32 add_by add_by_signs
-  in
-  let sums:Libcrux_intrinsics.Avx2_extract.t_Vec256 =
-    Libcrux_intrinsics.Avx2_extract.mm256_add_epi32 simd_unit add_by
-  in
-  let products:Libcrux_intrinsics.Avx2_extract.t_Vec256 =
-    Libcrux_ml_dsa.Simd.Avx2.Arithmetic.montgomery_multiply sums zetas
-  in
+  let add_by:u8 = Libcrux_intrinsics.Avx2_extract.mm256_shuffle_epi32 177l simd_unit in
+  let add_by:u8 = Libcrux_intrinsics.Avx2_extract.mm256_mullo_epi32 add_by add_by_signs in
+  let sums:u8 = Libcrux_intrinsics.Avx2_extract.mm256_add_epi32 simd_unit add_by in
+  let products:u8 = Libcrux_ml_dsa.Simd.Avx2.Arithmetic.montgomery_multiply sums zetas in
   Libcrux_intrinsics.Avx2_extract.mm256_blend_epi32 170l sums products
 
-let invert_ntt_at_layer_1_ (simd_unit: Libcrux_intrinsics.Avx2_extract.t_Vec256) (zeta0 zeta1: i32) =
-  let zetas:Libcrux_intrinsics.Avx2_extract.t_Vec256 =
+let invert_ntt_at_layer_1_ (simd_unit: u8) (zeta0 zeta1: i32) =
+  let zetas:u8 =
     Libcrux_intrinsics.Avx2_extract.mm256_set_epi32 zeta1 zeta1 0l 0l zeta0 zeta0 0l 0l
   in
-  let add_by_signs:Libcrux_intrinsics.Avx2_extract.t_Vec256 =
+  let add_by_signs:u8 =
     Libcrux_intrinsics.Avx2_extract.mm256_set_epi32 (-1l) (-1l) 1l 1l (-1l) (-1l) 1l 1l
   in
-  let add_by:Libcrux_intrinsics.Avx2_extract.t_Vec256 =
-    Libcrux_intrinsics.Avx2_extract.mm256_shuffle_epi32 78l simd_unit
-  in
-  let add_by:Libcrux_intrinsics.Avx2_extract.t_Vec256 =
-    Libcrux_intrinsics.Avx2_extract.mm256_mullo_epi32 add_by add_by_signs
-  in
-  let sums:Libcrux_intrinsics.Avx2_extract.t_Vec256 =
-    Libcrux_intrinsics.Avx2_extract.mm256_add_epi32 simd_unit add_by
-  in
-  let products:Libcrux_intrinsics.Avx2_extract.t_Vec256 =
-    Libcrux_ml_dsa.Simd.Avx2.Arithmetic.montgomery_multiply sums zetas
-  in
+  let add_by:u8 = Libcrux_intrinsics.Avx2_extract.mm256_shuffle_epi32 78l simd_unit in
+  let add_by:u8 = Libcrux_intrinsics.Avx2_extract.mm256_mullo_epi32 add_by add_by_signs in
+  let sums:u8 = Libcrux_intrinsics.Avx2_extract.mm256_add_epi32 simd_unit add_by in
+  let products:u8 = Libcrux_ml_dsa.Simd.Avx2.Arithmetic.montgomery_multiply sums zetas in
   Libcrux_intrinsics.Avx2_extract.mm256_blend_epi32 204l sums products
 
-let invert_ntt_at_layer_2_ (simd_unit: Libcrux_intrinsics.Avx2_extract.t_Vec256) (zeta: i32) =
-  let zetas:Libcrux_intrinsics.Avx2_extract.t_Vec256 =
-    Libcrux_intrinsics.Avx2_extract.mm256_set_epi32 zeta zeta zeta zeta 0l 0l 0l 0l
-  in
-  let add_by_signs:Libcrux_intrinsics.Avx2_extract.t_Vec256 =
+let invert_ntt_at_layer_2_ (simd_unit: u8) (zeta: i32) =
+  let zetas:u8 = Libcrux_intrinsics.Avx2_extract.mm256_set_epi32 zeta zeta zeta zeta 0l 0l 0l 0l in
+  let add_by_signs:u8 =
     Libcrux_intrinsics.Avx2_extract.mm256_set_epi32 (-1l) (-1l) (-1l) (-1l) 1l 1l 1l 1l
   in
-  let add_by:Libcrux_intrinsics.Avx2_extract.t_Vec256 =
-    Libcrux_intrinsics.Avx2_extract.mm256_permute4x64_epi64 78l simd_unit
-  in
-  let add_by:Libcrux_intrinsics.Avx2_extract.t_Vec256 =
-    Libcrux_intrinsics.Avx2_extract.mm256_mullo_epi32 add_by add_by_signs
-  in
-  let sums:Libcrux_intrinsics.Avx2_extract.t_Vec256 =
-    Libcrux_intrinsics.Avx2_extract.mm256_add_epi32 simd_unit add_by
-  in
-  let products:Libcrux_intrinsics.Avx2_extract.t_Vec256 =
-    Libcrux_ml_dsa.Simd.Avx2.Arithmetic.montgomery_multiply sums zetas
-  in
+  let add_by:u8 = Libcrux_intrinsics.Avx2_extract.mm256_permute4x64_epi64 78l simd_unit in
+  let add_by:u8 = Libcrux_intrinsics.Avx2_extract.mm256_mullo_epi32 add_by add_by_signs in
+  let sums:u8 = Libcrux_intrinsics.Avx2_extract.mm256_add_epi32 simd_unit add_by in
+  let products:u8 = Libcrux_ml_dsa.Simd.Avx2.Arithmetic.montgomery_multiply sums zetas in
   Libcrux_intrinsics.Avx2_extract.mm256_blend_epi32 240l sums products
 
-let ntt_at_layer_3_plus
-      (v_LAYER zeta_i: usize)
-      (re: t_Array Libcrux_intrinsics.Avx2_extract.t_Vec256 (sz 32))
-     =
+let ntt_at_layer_3_plus (v_LAYER zeta_i: usize) (re: t_Array u8 (sz 32)) =
   let step:usize = sz 1 <<! v_LAYER in
-  let re, zeta_i:(t_Array Libcrux_intrinsics.Avx2_extract.t_Vec256 (sz 32) & usize) =
+  let re, zeta_i:(t_Array u8 (sz 32) & usize) =
     Rust_primitives.Hax.Folds.fold_range (sz 0)
       (sz 128 >>! v_LAYER <: usize)
       (fun temp_0_ temp_1_ ->
-          let re, zeta_i:(t_Array Libcrux_intrinsics.Avx2_extract.t_Vec256 (sz 32) & usize) =
-            temp_0_
-          in
+          let re, zeta_i:(t_Array u8 (sz 32) & usize) = temp_0_ in
           let _:usize = temp_1_ in
           true)
-      (re, zeta_i <: (t_Array Libcrux_intrinsics.Avx2_extract.t_Vec256 (sz 32) & usize))
+      (re, zeta_i <: (t_Array u8 (sz 32) & usize))
       (fun temp_0_ round ->
-          let re, zeta_i:(t_Array Libcrux_intrinsics.Avx2_extract.t_Vec256 (sz 32) & usize) =
-            temp_0_
-          in
+          let re, zeta_i:(t_Array u8 (sz 32) & usize) = temp_0_ in
           let round:usize = round in
           let zeta_i:usize = zeta_i +! sz 1 in
           let offset:usize =
@@ -226,78 +140,59 @@ let ntt_at_layer_3_plus
             Libcrux_ml_dsa.Simd.Traits.v_COEFFICIENTS_IN_SIMD_UNIT
           in
           let step_by:usize = step /! Libcrux_ml_dsa.Simd.Traits.v_COEFFICIENTS_IN_SIMD_UNIT in
-          let re:t_Array Libcrux_intrinsics.Avx2_extract.t_Vec256 (sz 32) =
+          let re:t_Array u8 (sz 32) =
             Rust_primitives.Hax.Folds.fold_range offset
               (offset +! step_by <: usize)
               (fun re temp_1_ ->
-                  let re:t_Array Libcrux_intrinsics.Avx2_extract.t_Vec256 (sz 32) = re in
+                  let re:t_Array u8 (sz 32) = re in
                   let _:usize = temp_1_ in
                   true)
               re
               (fun re j ->
-                  let re:t_Array Libcrux_intrinsics.Avx2_extract.t_Vec256 (sz 32) = re in
+                  let re:t_Array u8 (sz 32) = re in
                   let j:usize = j in
-                  let t:Libcrux_intrinsics.Avx2_extract.t_Vec256 =
+                  let t:u8 =
                     Libcrux_ml_dsa.Simd.Avx2.Arithmetic.montgomery_multiply_by_constant (re.[ j +!
                           step_by
                           <:
                           usize ]
                         <:
-                        Libcrux_intrinsics.Avx2_extract.t_Vec256)
+                        u8)
                       (Libcrux_ml_dsa.Simd.Traits.v_ZETAS_TIMES_MONTGOMERY_R.[ zeta_i ] <: i32)
                   in
-                  let re:t_Array Libcrux_intrinsics.Avx2_extract.t_Vec256 (sz 32) =
+                  let re:t_Array u8 (sz 32) =
                     Rust_primitives.Hax.Monomorphized_update_at.update_at_usize re
                       (j +! step_by <: usize)
-                      (Libcrux_ml_dsa.Simd.Avx2.Arithmetic.subtract (re.[ j ]
-                            <:
-                            Libcrux_intrinsics.Avx2_extract.t_Vec256)
-                          t
-                        <:
-                        Libcrux_intrinsics.Avx2_extract.t_Vec256)
+                      (Libcrux_ml_dsa.Simd.Avx2.Arithmetic.subtract (re.[ j ] <: u8) t <: u8)
                   in
-                  let re:t_Array Libcrux_intrinsics.Avx2_extract.t_Vec256 (sz 32) =
+                  let re:t_Array u8 (sz 32) =
                     Rust_primitives.Hax.Monomorphized_update_at.update_at_usize re
                       j
-                      (Libcrux_ml_dsa.Simd.Avx2.Arithmetic.add (re.[ j ]
-                            <:
-                            Libcrux_intrinsics.Avx2_extract.t_Vec256)
-                          t
-                        <:
-                        Libcrux_intrinsics.Avx2_extract.t_Vec256)
+                      (Libcrux_ml_dsa.Simd.Avx2.Arithmetic.add (re.[ j ] <: u8) t <: u8)
                   in
                   re)
           in
-          re, zeta_i <: (t_Array Libcrux_intrinsics.Avx2_extract.t_Vec256 (sz 32) & usize))
+          re, zeta_i <: (t_Array u8 (sz 32) & usize))
   in
   let hax_temp_output:Prims.unit = () <: Prims.unit in
-  zeta_i, re <: (usize & t_Array Libcrux_intrinsics.Avx2_extract.t_Vec256 (sz 32))
+  zeta_i, re <: (usize & t_Array u8 (sz 32))
 
-let ntt_at_layer_0_ (zeta_i: usize) (re: t_Array Libcrux_intrinsics.Avx2_extract.t_Vec256 (sz 32)) =
+let ntt_at_layer_0_ (zeta_i: usize) (re: t_Array u8 (sz 32)) =
   let zeta_i:usize = zeta_i +! sz 1 in
-  let re, zeta_i:(t_Array Libcrux_intrinsics.Avx2_extract.t_Vec256 (sz 32) & usize) =
+  let re, zeta_i:(t_Array u8 (sz 32) & usize) =
     Rust_primitives.Hax.Folds.fold_range_step_by (sz 0)
-      (Core.Slice.impl__len #Libcrux_intrinsics.Avx2_extract.t_Vec256
-          (re <: t_Slice Libcrux_intrinsics.Avx2_extract.t_Vec256)
-        <:
-        usize)
+      (Core.Slice.impl__len #u8 (re <: t_Slice u8) <: usize)
       (sz 2)
       (fun temp_0_ temp_1_ ->
-          let re, zeta_i:(t_Array Libcrux_intrinsics.Avx2_extract.t_Vec256 (sz 32) & usize) =
-            temp_0_
-          in
+          let re, zeta_i:(t_Array u8 (sz 32) & usize) = temp_0_ in
           let _:usize = temp_1_ in
           true)
-      (re, zeta_i <: (t_Array Libcrux_intrinsics.Avx2_extract.t_Vec256 (sz 32) & usize))
+      (re, zeta_i <: (t_Array u8 (sz 32) & usize))
       (fun temp_0_ round ->
-          let re, zeta_i:(t_Array Libcrux_intrinsics.Avx2_extract.t_Vec256 (sz 32) & usize) =
-            temp_0_
-          in
+          let re, zeta_i:(t_Array u8 (sz 32) & usize) = temp_0_ in
           let round:usize = round in
-          let a, b:(Libcrux_intrinsics.Avx2_extract.t_Vec256 &
-            Libcrux_intrinsics.Avx2_extract.t_Vec256) =
-            butterfly_2_ (re.[ round ] <: Libcrux_intrinsics.Avx2_extract.t_Vec256)
-              (re.[ round +! sz 1 <: usize ] <: Libcrux_intrinsics.Avx2_extract.t_Vec256)
+          let a, b:(u8 & u8) =
+            butterfly_2_ (re.[ round ] <: u8) (re.[ round +! sz 1 <: usize ] <: u8)
               (Libcrux_ml_dsa.Simd.Traits.v_ZETAS_TIMES_MONTGOMERY_R.[ zeta_i ] <: i32)
               (Libcrux_ml_dsa.Simd.Traits.v_ZETAS_TIMES_MONTGOMERY_R.[ zeta_i +! sz 1 <: usize ]
                 <:
@@ -321,45 +216,37 @@ let ntt_at_layer_0_ (zeta_i: usize) (re: t_Array Libcrux_intrinsics.Avx2_extract
                 <:
                 i32)
           in
-          let re:t_Array Libcrux_intrinsics.Avx2_extract.t_Vec256 (sz 32) =
+          let re:t_Array u8 (sz 32) =
             Rust_primitives.Hax.Monomorphized_update_at.update_at_usize re round a
           in
-          let re:t_Array Libcrux_intrinsics.Avx2_extract.t_Vec256 (sz 32) =
+          let re:t_Array u8 (sz 32) =
             Rust_primitives.Hax.Monomorphized_update_at.update_at_usize re
               (round +! sz 1 <: usize)
               b
           in
           let zeta_i:usize = zeta_i +! sz 8 in
-          re, zeta_i <: (t_Array Libcrux_intrinsics.Avx2_extract.t_Vec256 (sz 32) & usize))
+          re, zeta_i <: (t_Array u8 (sz 32) & usize))
   in
   let zeta_i:usize = zeta_i -! sz 1 in
-  zeta_i, re <: (usize & t_Array Libcrux_intrinsics.Avx2_extract.t_Vec256 (sz 32))
+  zeta_i, re <: (usize & t_Array u8 (sz 32))
 
-let ntt_at_layer_1_ (zeta_i: usize) (re: t_Array Libcrux_intrinsics.Avx2_extract.t_Vec256 (sz 32)) =
+let ntt_at_layer_1_ (zeta_i: usize) (re: t_Array u8 (sz 32)) =
   let zeta_i:usize = zeta_i +! sz 1 in
-  let re, zeta_i:(t_Array Libcrux_intrinsics.Avx2_extract.t_Vec256 (sz 32) & usize) =
+  let re, zeta_i:(t_Array u8 (sz 32) & usize) =
     Rust_primitives.Hax.Folds.fold_range_step_by (sz 0)
-      (Core.Slice.impl__len #Libcrux_intrinsics.Avx2_extract.t_Vec256
-          (re <: t_Slice Libcrux_intrinsics.Avx2_extract.t_Vec256)
-        <:
-        usize)
+      (Core.Slice.impl__len #u8 (re <: t_Slice u8) <: usize)
       (sz 2)
       (fun temp_0_ temp_1_ ->
-          let re, zeta_i:(t_Array Libcrux_intrinsics.Avx2_extract.t_Vec256 (sz 32) & usize) =
-            temp_0_
-          in
+          let re, zeta_i:(t_Array u8 (sz 32) & usize) = temp_0_ in
           let _:usize = temp_1_ in
           true)
-      (re, zeta_i <: (t_Array Libcrux_intrinsics.Avx2_extract.t_Vec256 (sz 32) & usize))
+      (re, zeta_i <: (t_Array u8 (sz 32) & usize))
       (fun temp_0_ round ->
-          let re, zeta_i:(t_Array Libcrux_intrinsics.Avx2_extract.t_Vec256 (sz 32) & usize) =
-            temp_0_
-          in
+          let re, zeta_i:(t_Array u8 (sz 32) & usize) = temp_0_ in
           let round:usize = round in
-          let a, b:(Libcrux_intrinsics.Avx2_extract.t_Vec256 &
-            Libcrux_intrinsics.Avx2_extract.t_Vec256) =
-            butterfly_4_ (re.[ round ] <: Libcrux_intrinsics.Avx2_extract.t_Vec256)
-              (re.[ round +! sz 1 <: usize ] <: Libcrux_intrinsics.Avx2_extract.t_Vec256)
+          let a, b:(u8 & u8) =
+            butterfly_4_ (re.[ round ] <: u8)
+              (re.[ round +! sz 1 <: usize ] <: u8)
               (Libcrux_ml_dsa.Simd.Traits.v_ZETAS_TIMES_MONTGOMERY_R.[ zeta_i ] <: i32)
               (Libcrux_ml_dsa.Simd.Traits.v_ZETAS_TIMES_MONTGOMERY_R.[ zeta_i +! sz 1 <: usize ]
                 <:
@@ -371,112 +258,88 @@ let ntt_at_layer_1_ (zeta_i: usize) (re: t_Array Libcrux_intrinsics.Avx2_extract
                 <:
                 i32)
           in
-          let re:t_Array Libcrux_intrinsics.Avx2_extract.t_Vec256 (sz 32) =
+          let re:t_Array u8 (sz 32) =
             Rust_primitives.Hax.Monomorphized_update_at.update_at_usize re round a
           in
-          let re:t_Array Libcrux_intrinsics.Avx2_extract.t_Vec256 (sz 32) =
+          let re:t_Array u8 (sz 32) =
             Rust_primitives.Hax.Monomorphized_update_at.update_at_usize re
               (round +! sz 1 <: usize)
               b
           in
           let zeta_i:usize = zeta_i +! sz 4 in
-          re, zeta_i <: (t_Array Libcrux_intrinsics.Avx2_extract.t_Vec256 (sz 32) & usize))
+          re, zeta_i <: (t_Array u8 (sz 32) & usize))
   in
   let zeta_i:usize = zeta_i -! sz 1 in
-  zeta_i, re <: (usize & t_Array Libcrux_intrinsics.Avx2_extract.t_Vec256 (sz 32))
+  zeta_i, re <: (usize & t_Array u8 (sz 32))
 
-let ntt_at_layer_2_ (zeta_i: usize) (re: t_Array Libcrux_intrinsics.Avx2_extract.t_Vec256 (sz 32)) =
-  let re, zeta_i:(t_Array Libcrux_intrinsics.Avx2_extract.t_Vec256 (sz 32) & usize) =
+let ntt_at_layer_2_ (zeta_i: usize) (re: t_Array u8 (sz 32)) =
+  let re, zeta_i:(t_Array u8 (sz 32) & usize) =
     Rust_primitives.Hax.Folds.fold_range_step_by (sz 0)
-      (Core.Slice.impl__len #Libcrux_intrinsics.Avx2_extract.t_Vec256
-          (re <: t_Slice Libcrux_intrinsics.Avx2_extract.t_Vec256)
-        <:
-        usize)
+      (Core.Slice.impl__len #u8 (re <: t_Slice u8) <: usize)
       (sz 2)
       (fun temp_0_ temp_1_ ->
-          let re, zeta_i:(t_Array Libcrux_intrinsics.Avx2_extract.t_Vec256 (sz 32) & usize) =
-            temp_0_
-          in
+          let re, zeta_i:(t_Array u8 (sz 32) & usize) = temp_0_ in
           let _:usize = temp_1_ in
           true)
-      (re, zeta_i <: (t_Array Libcrux_intrinsics.Avx2_extract.t_Vec256 (sz 32) & usize))
+      (re, zeta_i <: (t_Array u8 (sz 32) & usize))
       (fun temp_0_ round ->
-          let re, zeta_i:(t_Array Libcrux_intrinsics.Avx2_extract.t_Vec256 (sz 32) & usize) =
-            temp_0_
-          in
+          let re, zeta_i:(t_Array u8 (sz 32) & usize) = temp_0_ in
           let round:usize = round in
           let zeta_i:usize = zeta_i +! sz 1 in
-          let a, b:(Libcrux_intrinsics.Avx2_extract.t_Vec256 &
-            Libcrux_intrinsics.Avx2_extract.t_Vec256) =
-            butterfly_8_ (re.[ round ] <: Libcrux_intrinsics.Avx2_extract.t_Vec256)
-              (re.[ round +! sz 1 <: usize ] <: Libcrux_intrinsics.Avx2_extract.t_Vec256)
+          let a, b:(u8 & u8) =
+            butterfly_8_ (re.[ round ] <: u8)
+              (re.[ round +! sz 1 <: usize ] <: u8)
               (Libcrux_ml_dsa.Simd.Traits.v_ZETAS_TIMES_MONTGOMERY_R.[ zeta_i ] <: i32)
               (Libcrux_ml_dsa.Simd.Traits.v_ZETAS_TIMES_MONTGOMERY_R.[ zeta_i +! sz 1 <: usize ]
                 <:
                 i32)
           in
-          let re:t_Array Libcrux_intrinsics.Avx2_extract.t_Vec256 (sz 32) =
+          let re:t_Array u8 (sz 32) =
             Rust_primitives.Hax.Monomorphized_update_at.update_at_usize re round a
           in
-          let re:t_Array Libcrux_intrinsics.Avx2_extract.t_Vec256 (sz 32) =
+          let re:t_Array u8 (sz 32) =
             Rust_primitives.Hax.Monomorphized_update_at.update_at_usize re
               (round +! sz 1 <: usize)
               b
           in
           let zeta_i:usize = zeta_i +! sz 1 in
-          re, zeta_i <: (t_Array Libcrux_intrinsics.Avx2_extract.t_Vec256 (sz 32) & usize))
+          re, zeta_i <: (t_Array u8 (sz 32) & usize))
   in
   let hax_temp_output:Prims.unit = () <: Prims.unit in
-  zeta_i, re <: (usize & t_Array Libcrux_intrinsics.Avx2_extract.t_Vec256 (sz 32))
+  zeta_i, re <: (usize & t_Array u8 (sz 32))
 
-let ntt (re: t_Array Libcrux_intrinsics.Avx2_extract.t_Vec256 (sz 32)) =
+let ntt (re: t_Array u8 (sz 32)) =
   let zeta_i:usize = sz 0 in
-  let tmp0, tmp1:(usize & t_Array Libcrux_intrinsics.Avx2_extract.t_Vec256 (sz 32)) =
-    ntt_at_layer_3_plus (sz 7) zeta_i re
-  in
+  let tmp0, tmp1:(usize & t_Array u8 (sz 32)) = ntt_at_layer_3_plus (sz 7) zeta_i re in
   let zeta_i:usize = tmp0 in
-  let re:t_Array Libcrux_intrinsics.Avx2_extract.t_Vec256 (sz 32) = tmp1 in
+  let re:t_Array u8 (sz 32) = tmp1 in
   let _:Prims.unit = () in
-  let tmp0, tmp1:(usize & t_Array Libcrux_intrinsics.Avx2_extract.t_Vec256 (sz 32)) =
-    ntt_at_layer_3_plus (sz 6) zeta_i re
-  in
+  let tmp0, tmp1:(usize & t_Array u8 (sz 32)) = ntt_at_layer_3_plus (sz 6) zeta_i re in
   let zeta_i:usize = tmp0 in
-  let re:t_Array Libcrux_intrinsics.Avx2_extract.t_Vec256 (sz 32) = tmp1 in
+  let re:t_Array u8 (sz 32) = tmp1 in
   let _:Prims.unit = () in
-  let tmp0, tmp1:(usize & t_Array Libcrux_intrinsics.Avx2_extract.t_Vec256 (sz 32)) =
-    ntt_at_layer_3_plus (sz 5) zeta_i re
-  in
+  let tmp0, tmp1:(usize & t_Array u8 (sz 32)) = ntt_at_layer_3_plus (sz 5) zeta_i re in
   let zeta_i:usize = tmp0 in
-  let re:t_Array Libcrux_intrinsics.Avx2_extract.t_Vec256 (sz 32) = tmp1 in
+  let re:t_Array u8 (sz 32) = tmp1 in
   let _:Prims.unit = () in
-  let tmp0, tmp1:(usize & t_Array Libcrux_intrinsics.Avx2_extract.t_Vec256 (sz 32)) =
-    ntt_at_layer_3_plus (sz 4) zeta_i re
-  in
+  let tmp0, tmp1:(usize & t_Array u8 (sz 32)) = ntt_at_layer_3_plus (sz 4) zeta_i re in
   let zeta_i:usize = tmp0 in
-  let re:t_Array Libcrux_intrinsics.Avx2_extract.t_Vec256 (sz 32) = tmp1 in
+  let re:t_Array u8 (sz 32) = tmp1 in
   let _:Prims.unit = () in
-  let tmp0, tmp1:(usize & t_Array Libcrux_intrinsics.Avx2_extract.t_Vec256 (sz 32)) =
-    ntt_at_layer_3_plus (sz 3) zeta_i re
-  in
+  let tmp0, tmp1:(usize & t_Array u8 (sz 32)) = ntt_at_layer_3_plus (sz 3) zeta_i re in
   let zeta_i:usize = tmp0 in
-  let re:t_Array Libcrux_intrinsics.Avx2_extract.t_Vec256 (sz 32) = tmp1 in
+  let re:t_Array u8 (sz 32) = tmp1 in
   let _:Prims.unit = () in
-  let tmp0, tmp1:(usize & t_Array Libcrux_intrinsics.Avx2_extract.t_Vec256 (sz 32)) =
-    ntt_at_layer_2_ zeta_i re
-  in
+  let tmp0, tmp1:(usize & t_Array u8 (sz 32)) = ntt_at_layer_2_ zeta_i re in
   let zeta_i:usize = tmp0 in
-  let re:t_Array Libcrux_intrinsics.Avx2_extract.t_Vec256 (sz 32) = tmp1 in
+  let re:t_Array u8 (sz 32) = tmp1 in
   let _:Prims.unit = () in
-  let tmp0, tmp1:(usize & t_Array Libcrux_intrinsics.Avx2_extract.t_Vec256 (sz 32)) =
-    ntt_at_layer_1_ zeta_i re
-  in
+  let tmp0, tmp1:(usize & t_Array u8 (sz 32)) = ntt_at_layer_1_ zeta_i re in
   let zeta_i:usize = tmp0 in
-  let re:t_Array Libcrux_intrinsics.Avx2_extract.t_Vec256 (sz 32) = tmp1 in
+  let re:t_Array u8 (sz 32) = tmp1 in
   let _:Prims.unit = () in
-  let tmp0, tmp1:(usize & t_Array Libcrux_intrinsics.Avx2_extract.t_Vec256 (sz 32)) =
-    ntt_at_layer_0_ zeta_i re
-  in
+  let tmp0, tmp1:(usize & t_Array u8 (sz 32)) = ntt_at_layer_0_ zeta_i re in
   let zeta_i:usize = tmp0 in
-  let re:t_Array Libcrux_intrinsics.Avx2_extract.t_Vec256 (sz 32) = tmp1 in
+  let re:t_Array u8 (sz 32) = tmp1 in
   let _:Prims.unit = () in
   re
