libcrux-ml-dsa/proofs/fstar/extraction/Libcrux_ml_dsa.Simd.Avx2.Vector_type.fst
@@ -4,20 +4,16 @@ open Core
 open FStar.Mul
 
 let v_ZERO (_: Prims.unit) =
-  Core.Convert.f_into #Libcrux_intrinsics.Avx2_extract.t_Vec256
+  Core.Convert.f_into #u8
     #t_AVX2SIMDUnit
     #FStar.Tactics.Typeclasses.solve
-    (Libcrux_intrinsics.Avx2_extract.mm256_setzero_si256 ()
-      <:
-      Libcrux_intrinsics.Avx2_extract.t_Vec256)
+    (Libcrux_intrinsics.Avx2_extract.mm256_setzero_si256 () <: u8)
 
 let from_coefficient_array (coefficient_array: t_Slice i32) =
-  Core.Convert.f_into #Libcrux_intrinsics.Avx2_extract.t_Vec256
+  Core.Convert.f_into #u8
     #t_AVX2SIMDUnit
     #FStar.Tactics.Typeclasses.solve
-    (Libcrux_intrinsics.Avx2_extract.mm256_loadu_si256_i32 coefficient_array
-      <:
-      Libcrux_intrinsics.Avx2_extract.t_Vec256)
+    (Libcrux_intrinsics.Avx2_extract.mm256_loadu_si256_i32 coefficient_array <: u8)
 
 let to_coefficient_array (x: t_AVX2SIMDUnit) =
   let coefficient_array:t_Array i32 (sz 8) = Rust_primitives.Hax.repeat 0l (sz 8) in
